Début d'une version où tout est indicé.

src/HOL/Base.v
@@ -1,996 +1,1224 @@
-Require Import core unscoped.
+Require Import core fintype.
 
 Require Import Setoid Morphisms Relation_Definitions.
 
 
 Module Core.
 
-Inductive st : Type :=
-| nat_st : st
-| bool_st : st
-| list_st : st -> st
-| prop_st : st
-| to_st : st -> st -> st
-| prod_st : st -> st -> st.
-
-Notation ℕₛ := nat_st.
-Notation 𝔹ₛ := bool_st.
-Notation 𝕃ₛ := list_st.
-Notation ℙₛ := prop_st.
-Notation "s →ₛ s'" := (to_st s s') (at level 86, right associativity).
-Notation "s ×ₛ s'" := (prod_st s s') (at level 86, right associativity).
-
-Lemma congr_nat_st : nat_st = nat_st.
-Proof.
-exact (eq_refl).
-Qed.
-
-Lemma congr_bool_st : bool_st = bool_st.
-Proof.
-exact (eq_refl).
-Qed.
-
-Lemma congr_list_st {s0 : st} {t0 : st} (H0 : s0 = t0) :
-  list_st s0 = list_st t0.
-Proof.
-exact (eq_trans eq_refl (ap (fun x => list_st x) H0)).
-Qed.
-
-Lemma congr_prop_st : prop_st = prop_st.
-Proof.
-exact (eq_refl).
-Qed.
-
-Lemma congr_to_st {s0 : st} {s1 : st} {t0 : st} {t1 : st} (H0 : s0 = t0)
-  (H1 : s1 = t1) : to_st s0 s1 = to_st t0 t1.
-Proof.
-exact (eq_trans (eq_trans eq_refl (ap (fun x => to_st x s1) H0))
-         (ap (fun x => to_st t0 x) H1)).
-Qed.
-
-Lemma congr_prod_st {s0 : st} {s1 : st} {t0 : st} {t1 : st} (H0 : s0 = t0)
-  (H1 : s1 = t1) : prod_st s0 s1 = prod_st t0 t1.
-Proof.
-exact (eq_trans (eq_trans eq_refl (ap (fun x => prod_st x s1) H0))
-         (ap (fun x => prod_st t0 x) H1)).
-Qed.
-
-Inductive tm : Type :=
-| var_tm : nat -> tm
-| lam_tm : tm -> tm
-| app_tm : tm -> tm -> tm
-| z_tm : tm
-| s_tm : tm -> tm
-| recN_tm : tm -> tm -> tm -> tm
-| tt_tm : tm
-| ff_tm : tm
-| recB_tm : tm -> tm -> tm -> tm
-| nil_tm : tm
-| cons_tm : tm -> tm -> tm
-| recL_tm : tm -> tm -> tm -> tm
-| pair_tm : tm -> tm -> tm
-| pi1_tm : tm -> tm
-| pi2_tm : tm -> tm
-| imp_tm : tm -> tm -> tm
-| forall_tm : tm -> tm
-| sort_tm : tm -> tm.
-
-Notation "⟦ n ⟧ₛ" := (var_tm n).
-Notation ƛ := lam_tm.
-Notation "t @ₛ u" := (app_tm t u) (at level 88, left associativity).
-Notation Zₛ := z_tm.
-Notation Sₛ := s_tm.
-Notation recℕₛ := recN_tm.
-Notation ttₛ := tt_tm.
-Notation ffₛ := ff_tm.
-Notation rec𝔹ₛ := recB_tm.
-Notation "[]ₛ" := nil_tm.
-Notation "t ::ₛ u" := (cons_tm t u) (at level 86, right associativity).
-Notation rec𝕃ₛ := recL_tm.
-Notation "⟨ t , u ⟩ₛ" := (pair_tm t u).
-Notation "π¹ₛ" := pi1_tm.
-Notation "π²ₛ" := pi2_tm.
-Notation "φ ⇒ₛ ψ" := (imp_tm φ ψ) (at level 89, right associativity).
-Notation "∀ₛ" := forall_tm.
-Notation 𝕊 := sort_tm.
-
-Lemma congr_lam_tm {s0 : tm} {t0 : tm} (H0 : s0 = t0) : lam_tm s0 = lam_tm t0.
-Proof.
-exact (eq_trans eq_refl (ap (fun x => lam_tm x) H0)).
-Qed.
-
-Lemma congr_app_tm {s0 : tm} {s1 : tm} {t0 : tm} {t1 : tm} (H0 : s0 = t0)
-  (H1 : s1 = t1) : app_tm s0 s1 = app_tm t0 t1.
-Proof.
-exact (eq_trans (eq_trans eq_refl (ap (fun x => app_tm x s1) H0))
-         (ap (fun x => app_tm t0 x) H1)).
-Qed.
-
-Lemma congr_z_tm : z_tm = z_tm.
-Proof.
-exact (eq_refl).
-Qed.
-
-Lemma congr_s_tm {s0 : tm} {t0 : tm} (H0 : s0 = t0) : s_tm s0 = s_tm t0.
-Proof.
-exact (eq_trans eq_refl (ap (fun x => s_tm x) H0)).
-Qed.
-
-Lemma congr_recN_tm {s0 : tm} {s1 : tm} {s2 : tm} {t0 : tm} {t1 : tm}
-  {t2 : tm} (H0 : s0 = t0) (H1 : s1 = t1) (H2 : s2 = t2) :
-  recN_tm s0 s1 s2 = recN_tm t0 t1 t2.
-Proof.
-exact (eq_trans
-         (eq_trans (eq_trans eq_refl (ap (fun x => recN_tm x s1 s2) H0))
-            (ap (fun x => recN_tm t0 x s2) H1))
-         (ap (fun x => recN_tm t0 t1 x) H2)).
-Qed.
-
-Lemma congr_tt_tm : tt_tm = tt_tm.
-Proof.
-exact (eq_refl).
-Qed.
-
-Lemma congr_ff_tm : ff_tm = ff_tm.
-Proof.
-exact (eq_refl).
-Qed.
-
-Lemma congr_recB_tm {s0 : tm} {s1 : tm} {s2 : tm} {t0 : tm} {t1 : tm}
-  {t2 : tm} (H0 : s0 = t0) (H1 : s1 = t1) (H2 : s2 = t2) :
-  recB_tm s0 s1 s2 = recB_tm t0 t1 t2.
-Proof.
-exact (eq_trans
-         (eq_trans (eq_trans eq_refl (ap (fun x => recB_tm x s1 s2) H0))
-            (ap (fun x => recB_tm t0 x s2) H1))
-         (ap (fun x => recB_tm t0 t1 x) H2)).
-Qed.
-
-Lemma congr_nil_tm : nil_tm = nil_tm.
-Proof.
-exact (eq_refl).
-Qed.
-
-Lemma congr_cons_tm {s0 : tm} {s1 : tm} {t0 : tm} {t1 : tm} (H0 : s0 = t0)
-  (H1 : s1 = t1) : cons_tm s0 s1 = cons_tm t0 t1.
-Proof.
-exact (eq_trans (eq_trans eq_refl (ap (fun x => cons_tm x s1) H0))
-         (ap (fun x => cons_tm t0 x) H1)).
-Qed.
-
-Lemma congr_recL_tm {s0 : tm} {s1 : tm} {s2 : tm} {t0 : tm} {t1 : tm}
-  {t2 : tm} (H0 : s0 = t0) (H1 : s1 = t1) (H2 : s2 = t2) :
-  recL_tm s0 s1 s2 = recL_tm t0 t1 t2.
-Proof.
-exact (eq_trans
-         (eq_trans (eq_trans eq_refl (ap (fun x => recL_tm x s1 s2) H0))
-            (ap (fun x => recL_tm t0 x s2) H1))
-         (ap (fun x => recL_tm t0 t1 x) H2)).
-Qed.
-
-Lemma congr_pair_tm {s0 : tm} {s1 : tm} {t0 : tm} {t1 : tm} (H0 : s0 = t0)
-  (H1 : s1 = t1) : pair_tm s0 s1 = pair_tm t0 t1.
-Proof.
-exact (eq_trans (eq_trans eq_refl (ap (fun x => pair_tm x s1) H0))
-         (ap (fun x => pair_tm t0 x) H1)).
-Qed.
-
-Lemma congr_pi1_tm {s0 : tm} {t0 : tm} (H0 : s0 = t0) : pi1_tm s0 = pi1_tm t0.
-Proof.
-exact (eq_trans eq_refl (ap (fun x => pi1_tm x) H0)).
-Qed.
-
-Lemma congr_pi2_tm {s0 : tm} {t0 : tm} (H0 : s0 = t0) : pi2_tm s0 = pi2_tm t0.
-Proof.
-exact (eq_trans eq_refl (ap (fun x => pi2_tm x) H0)).
-Qed.
-
-Lemma congr_imp_tm {s0 : tm} {s1 : tm} {t0 : tm} {t1 : tm} (H0 : s0 = t0)
-  (H1 : s1 = t1) : imp_tm s0 s1 = imp_tm t0 t1.
-Proof.
-exact (eq_trans (eq_trans eq_refl (ap (fun x => imp_tm x s1) H0))
-         (ap (fun x => imp_tm t0 x) H1)).
-Qed.
-
-Lemma congr_forall_tm {s0 : tm} {t0 : tm} (H0 : s0 = t0) :
-  forall_tm s0 = forall_tm t0.
-Proof.
-exact (eq_trans eq_refl (ap (fun x => forall_tm x) H0)).
-Qed.
-
-Lemma congr_sort_tm {s0 : tm} {t0 : tm} (H0 : s0 = t0) :
-  sort_tm s0 = sort_tm t0.
-Proof.
-exact (eq_trans eq_refl (ap (fun x => sort_tm x) H0)).
-Qed.
-
-Lemma upRen_tm_tm (xi : nat -> nat) : nat -> nat.
-Proof.
-exact (up_ren xi).
-Defined.
-
-Fixpoint ren_tm (xi_tm : nat -> nat) (s : tm) {struct s} : tm :=
-  match s with
-  | var_tm s0 => var_tm (xi_tm s0)
-  | lam_tm s0 => lam_tm (ren_tm (upRen_tm_tm xi_tm) s0)
-  | app_tm s0 s1 => app_tm (ren_tm xi_tm s0) (ren_tm xi_tm s1)
-  | z_tm => z_tm
-  | s_tm s0 => s_tm (ren_tm xi_tm s0)
-  | recN_tm s0 s1 s2 =>
-      recN_tm (ren_tm xi_tm s0) (ren_tm xi_tm s1) (ren_tm xi_tm s2)
-  | tt_tm => tt_tm
-  | ff_tm => ff_tm
-  | recB_tm s0 s1 s2 =>
-      recB_tm (ren_tm xi_tm s0) (ren_tm xi_tm s1) (ren_tm xi_tm s2)
-  | nil_tm => nil_tm
-  | cons_tm s0 s1 => cons_tm (ren_tm xi_tm s0) (ren_tm xi_tm s1)
-  | recL_tm s0 s1 s2 =>
-      recL_tm (ren_tm xi_tm s0) (ren_tm xi_tm s1) (ren_tm xi_tm s2)
-  | pair_tm s0 s1 => pair_tm (ren_tm xi_tm s0) (ren_tm xi_tm s1)
-  | pi1_tm s0 => pi1_tm (ren_tm xi_tm s0)
-  | pi2_tm s0 => pi2_tm (ren_tm xi_tm s0)
-  | imp_tm s0 s1 => imp_tm (ren_tm xi_tm s0) (ren_tm xi_tm s1)
-  | forall_tm s0 => forall_tm (ren_tm (upRen_tm_tm xi_tm) s0)
-  | sort_tm s0 => sort_tm (ren_tm xi_tm s0)
-  end.
-
-Lemma up_tm_tm (sigma : nat -> tm) : nat -> tm.
-Proof.
-exact (scons (var_tm var_zero) (funcomp (ren_tm shift) sigma)).
-Defined.
-
-Fixpoint subst_tm (sigma_tm : nat -> tm) (s : tm) {struct s} : tm :=
-  match s with
-  | var_tm s0 => sigma_tm s0
-  | lam_tm s0 => lam_tm (subst_tm (up_tm_tm sigma_tm) s0)
-  | app_tm s0 s1 => app_tm (subst_tm sigma_tm s0) (subst_tm sigma_tm s1)
-  | z_tm => z_tm
-  | s_tm s0 => s_tm (subst_tm sigma_tm s0)
-  | recN_tm s0 s1 s2 =>
-      recN_tm (subst_tm sigma_tm s0) (subst_tm sigma_tm s1)
-        (subst_tm sigma_tm s2)
-  | tt_tm => tt_tm
-  | ff_tm => ff_tm
-  | recB_tm s0 s1 s2 =>
-      recB_tm (subst_tm sigma_tm s0) (subst_tm sigma_tm s1)
-        (subst_tm sigma_tm s2)
-  | nil_tm => nil_tm
-  | cons_tm s0 s1 => cons_tm (subst_tm sigma_tm s0) (subst_tm sigma_tm s1)
-  | recL_tm s0 s1 s2 =>
-      recL_tm (subst_tm sigma_tm s0) (subst_tm sigma_tm s1)
-        (subst_tm sigma_tm s2)
-  | pair_tm s0 s1 => pair_tm (subst_tm sigma_tm s0) (subst_tm sigma_tm s1)
-  | pi1_tm s0 => pi1_tm (subst_tm sigma_tm s0)
-  | pi2_tm s0 => pi2_tm (subst_tm sigma_tm s0)
-  | imp_tm s0 s1 => imp_tm (subst_tm sigma_tm s0) (subst_tm sigma_tm s1)
-  | forall_tm s0 => forall_tm (subst_tm (up_tm_tm sigma_tm) s0)
-  | sort_tm s0 => sort_tm (subst_tm sigma_tm s0)
-  end.
-
-Lemma upId_tm_tm (sigma : nat -> tm) (Eq : forall x, sigma x = var_tm x) :
-  forall x, up_tm_tm sigma x = var_tm x.
-Proof.
-exact (fun n =>
-       match n with
-       | S n' => ap (ren_tm shift) (Eq n')
-       | O => eq_refl
-       end).
-Qed.
-
-Fixpoint idSubst_tm (sigma_tm : nat -> tm)
-(Eq_tm : forall x, sigma_tm x = var_tm x) (s : tm) {struct s} :
-subst_tm sigma_tm s = s :=
-  match s with
-  | var_tm s0 => Eq_tm s0
-  | lam_tm s0 =>
-      congr_lam_tm (idSubst_tm (up_tm_tm sigma_tm) (upId_tm_tm _ Eq_tm) s0)
-  | app_tm s0 s1 =>
-      congr_app_tm (idSubst_tm sigma_tm Eq_tm s0)
-        (idSubst_tm sigma_tm Eq_tm s1)
-  | z_tm => congr_z_tm
-  | s_tm s0 => congr_s_tm (idSubst_tm sigma_tm Eq_tm s0)
-  | recN_tm s0 s1 s2 =>
-      congr_recN_tm (idSubst_tm sigma_tm Eq_tm s0)
-        (idSubst_tm sigma_tm Eq_tm s1) (idSubst_tm sigma_tm Eq_tm s2)
-  | tt_tm => congr_tt_tm
-  | ff_tm => congr_ff_tm
-  | recB_tm s0 s1 s2 =>
-      congr_recB_tm (idSubst_tm sigma_tm Eq_tm s0)
-        (idSubst_tm sigma_tm Eq_tm s1) (idSubst_tm sigma_tm Eq_tm s2)
-  | nil_tm => congr_nil_tm
-  | cons_tm s0 s1 =>
-      congr_cons_tm (idSubst_tm sigma_tm Eq_tm s0)
-        (idSubst_tm sigma_tm Eq_tm s1)
-  | recL_tm s0 s1 s2 =>
-      congr_recL_tm (idSubst_tm sigma_tm Eq_tm s0)
-        (idSubst_tm sigma_tm Eq_tm s1) (idSubst_tm sigma_tm Eq_tm s2)
-  | pair_tm s0 s1 =>
-      congr_pair_tm (idSubst_tm sigma_tm Eq_tm s0)
-        (idSubst_tm sigma_tm Eq_tm s1)
-  | pi1_tm s0 => congr_pi1_tm (idSubst_tm sigma_tm Eq_tm s0)
-  | pi2_tm s0 => congr_pi2_tm (idSubst_tm sigma_tm Eq_tm s0)
-  | imp_tm s0 s1 =>
-      congr_imp_tm (idSubst_tm sigma_tm Eq_tm s0)
-        (idSubst_tm sigma_tm Eq_tm s1)
-  | forall_tm s0 =>
-      congr_forall_tm
-        (idSubst_tm (up_tm_tm sigma_tm) (upId_tm_tm _ Eq_tm) s0)
-  | sort_tm s0 => congr_sort_tm (idSubst_tm sigma_tm Eq_tm s0)
-  end.
-
-Lemma upExtRen_tm_tm (xi : nat -> nat) (zeta : nat -> nat)
-  (Eq : forall x, xi x = zeta x) :
-  forall x, upRen_tm_tm xi x = upRen_tm_tm zeta x.
-Proof.
-exact (fun n => match n with
-                | S n' => ap shift (Eq n')
-                | O => eq_refl
-                end).
-Qed.
-
-Fixpoint extRen_tm (xi_tm : nat -> nat) (zeta_tm : nat -> nat)
-(Eq_tm : forall x, xi_tm x = zeta_tm x) (s : tm) {struct s} :
-ren_tm xi_tm s = ren_tm zeta_tm s :=
-  match s with
-  | var_tm s0 => ap (var_tm) (Eq_tm s0)
-  | lam_tm s0 =>
-      congr_lam_tm
-        (extRen_tm (upRen_tm_tm xi_tm) (upRen_tm_tm zeta_tm)
-           (upExtRen_tm_tm _ _ Eq_tm) s0)
-  | app_tm s0 s1 =>
-      congr_app_tm (extRen_tm xi_tm zeta_tm Eq_tm s0)
-        (extRen_tm xi_tm zeta_tm Eq_tm s1)
-  | z_tm => congr_z_tm
-  | s_tm s0 => congr_s_tm (extRen_tm xi_tm zeta_tm Eq_tm s0)
-  | recN_tm s0 s1 s2 =>
-      congr_recN_tm (extRen_tm xi_tm zeta_tm Eq_tm s0)
-        (extRen_tm xi_tm zeta_tm Eq_tm s1) (extRen_tm xi_tm zeta_tm Eq_tm s2)
-  | tt_tm => congr_tt_tm
-  | ff_tm => congr_ff_tm
-  | recB_tm s0 s1 s2 =>
-      congr_recB_tm (extRen_tm xi_tm zeta_tm Eq_tm s0)
-        (extRen_tm xi_tm zeta_tm Eq_tm s1) (extRen_tm xi_tm zeta_tm Eq_tm s2)
-  | nil_tm => congr_nil_tm
-  | cons_tm s0 s1 =>
-      congr_cons_tm (extRen_tm xi_tm zeta_tm Eq_tm s0)
-        (extRen_tm xi_tm zeta_tm Eq_tm s1)
-  | recL_tm s0 s1 s2 =>
-      congr_recL_tm (extRen_tm xi_tm zeta_tm Eq_tm s0)
-        (extRen_tm xi_tm zeta_tm Eq_tm s1) (extRen_tm xi_tm zeta_tm Eq_tm s2)
-  | pair_tm s0 s1 =>
-      congr_pair_tm (extRen_tm xi_tm zeta_tm Eq_tm s0)
-        (extRen_tm xi_tm zeta_tm Eq_tm s1)
-  | pi1_tm s0 => congr_pi1_tm (extRen_tm xi_tm zeta_tm Eq_tm s0)
-  | pi2_tm s0 => congr_pi2_tm (extRen_tm xi_tm zeta_tm Eq_tm s0)
-  | imp_tm s0 s1 =>
-      congr_imp_tm (extRen_tm xi_tm zeta_tm Eq_tm s0)
-        (extRen_tm xi_tm zeta_tm Eq_tm s1)
-  | forall_tm s0 =>
-      congr_forall_tm
-        (extRen_tm (upRen_tm_tm xi_tm) (upRen_tm_tm zeta_tm)
-           (upExtRen_tm_tm _ _ Eq_tm) s0)
-  | sort_tm s0 => congr_sort_tm (extRen_tm xi_tm zeta_tm Eq_tm s0)
-  end.
-
-Lemma upExt_tm_tm (sigma : nat -> tm) (tau : nat -> tm)
-  (Eq : forall x, sigma x = tau x) :
-  forall x, up_tm_tm sigma x = up_tm_tm tau x.
-Proof.
-exact (fun n =>
-       match n with
-       | S n' => ap (ren_tm shift) (Eq n')
-       | O => eq_refl
-       end).
-Qed.
-
-Fixpoint ext_tm (sigma_tm : nat -> tm) (tau_tm : nat -> tm)
-(Eq_tm : forall x, sigma_tm x = tau_tm x) (s : tm) {struct s} :
-subst_tm sigma_tm s = subst_tm tau_tm s :=
-  match s with
-  | var_tm s0 => Eq_tm s0
-  | lam_tm s0 =>
-      congr_lam_tm
-        (ext_tm (up_tm_tm sigma_tm) (up_tm_tm tau_tm) (upExt_tm_tm _ _ Eq_tm)
-           s0)
-  | app_tm s0 s1 =>
-      congr_app_tm (ext_tm sigma_tm tau_tm Eq_tm s0)
-        (ext_tm sigma_tm tau_tm Eq_tm s1)
-  | z_tm => congr_z_tm
-  | s_tm s0 => congr_s_tm (ext_tm sigma_tm tau_tm Eq_tm s0)
-  | recN_tm s0 s1 s2 =>
-      congr_recN_tm (ext_tm sigma_tm tau_tm Eq_tm s0)
-        (ext_tm sigma_tm tau_tm Eq_tm s1) (ext_tm sigma_tm tau_tm Eq_tm s2)
-  | tt_tm => congr_tt_tm
-  | ff_tm => congr_ff_tm
-  | recB_tm s0 s1 s2 =>
-      congr_recB_tm (ext_tm sigma_tm tau_tm Eq_tm s0)
-        (ext_tm sigma_tm tau_tm Eq_tm s1) (ext_tm sigma_tm tau_tm Eq_tm s2)
-  | nil_tm => congr_nil_tm
-  | cons_tm s0 s1 =>
-      congr_cons_tm (ext_tm sigma_tm tau_tm Eq_tm s0)
-        (ext_tm sigma_tm tau_tm Eq_tm s1)
-  | recL_tm s0 s1 s2 =>
-      congr_recL_tm (ext_tm sigma_tm tau_tm Eq_tm s0)
-        (ext_tm sigma_tm tau_tm Eq_tm s1) (ext_tm sigma_tm tau_tm Eq_tm s2)
-  | pair_tm s0 s1 =>
-      congr_pair_tm (ext_tm sigma_tm tau_tm Eq_tm s0)
-        (ext_tm sigma_tm tau_tm Eq_tm s1)
-  | pi1_tm s0 => congr_pi1_tm (ext_tm sigma_tm tau_tm Eq_tm s0)
-  | pi2_tm s0 => congr_pi2_tm (ext_tm sigma_tm tau_tm Eq_tm s0)
-  | imp_tm s0 s1 =>
-      congr_imp_tm (ext_tm sigma_tm tau_tm Eq_tm s0)
-        (ext_tm sigma_tm tau_tm Eq_tm s1)
-  | forall_tm s0 =>
-      congr_forall_tm
-        (ext_tm (up_tm_tm sigma_tm) (up_tm_tm tau_tm) (upExt_tm_tm _ _ Eq_tm)
-           s0)
-  | sort_tm s0 => congr_sort_tm (ext_tm sigma_tm tau_tm Eq_tm s0)
-  end.
-
-Lemma up_ren_ren_tm_tm (xi : nat -> nat) (zeta : nat -> nat)
-  (rho : nat -> nat) (Eq : forall x, funcomp zeta xi x = rho x) :
-  forall x, funcomp (upRen_tm_tm zeta) (upRen_tm_tm xi) x = upRen_tm_tm rho x.
-Proof.
-exact (up_ren_ren xi zeta rho Eq).
-Qed.
-
-Fixpoint compRenRen_tm (xi_tm : nat -> nat) (zeta_tm : nat -> nat)
-(rho_tm : nat -> nat) (Eq_tm : forall x, funcomp zeta_tm xi_tm x = rho_tm x)
-(s : tm) {struct s} : ren_tm zeta_tm (ren_tm xi_tm s) = ren_tm rho_tm s :=
-  match s with
-  | var_tm s0 => ap (var_tm) (Eq_tm s0)
-  | lam_tm s0 =>
-      congr_lam_tm
-        (compRenRen_tm (upRen_tm_tm xi_tm) (upRen_tm_tm zeta_tm)
-           (upRen_tm_tm rho_tm) (up_ren_ren _ _ _ Eq_tm) s0)
-  | app_tm s0 s1 =>
-      congr_app_tm (compRenRen_tm xi_tm zeta_tm rho_tm Eq_tm s0)
-        (compRenRen_tm xi_tm zeta_tm rho_tm Eq_tm s1)
-  | z_tm => congr_z_tm
-  | s_tm s0 => congr_s_tm (compRenRen_tm xi_tm zeta_tm rho_tm Eq_tm s0)
-  | recN_tm s0 s1 s2 =>
-      congr_recN_tm (compRenRen_tm xi_tm zeta_tm rho_tm Eq_tm s0)
-        (compRenRen_tm xi_tm zeta_tm rho_tm Eq_tm s1)
-        (compRenRen_tm xi_tm zeta_tm rho_tm Eq_tm s2)
-  | tt_tm => congr_tt_tm
-  | ff_tm => congr_ff_tm
-  | recB_tm s0 s1 s2 =>
-      congr_recB_tm (compRenRen_tm xi_tm zeta_tm rho_tm Eq_tm s0)
-        (compRenRen_tm xi_tm zeta_tm rho_tm Eq_tm s1)
-        (compRenRen_tm xi_tm zeta_tm rho_tm Eq_tm s2)
-  | nil_tm => congr_nil_tm
-  | cons_tm s0 s1 =>
-      congr_cons_tm (compRenRen_tm xi_tm zeta_tm rho_tm Eq_tm s0)
-        (compRenRen_tm xi_tm zeta_tm rho_tm Eq_tm s1)
-  | recL_tm s0 s1 s2 =>
-      congr_recL_tm (compRenRen_tm xi_tm zeta_tm rho_tm Eq_tm s0)
-        (compRenRen_tm xi_tm zeta_tm rho_tm Eq_tm s1)
-        (compRenRen_tm xi_tm zeta_tm rho_tm Eq_tm s2)
-  | pair_tm s0 s1 =>
-      congr_pair_tm (compRenRen_tm xi_tm zeta_tm rho_tm Eq_tm s0)
-        (compRenRen_tm xi_tm zeta_tm rho_tm Eq_tm s1)
-  | pi1_tm s0 => congr_pi1_tm (compRenRen_tm xi_tm zeta_tm rho_tm Eq_tm s0)
-  | pi2_tm s0 => congr_pi2_tm (compRenRen_tm xi_tm zeta_tm rho_tm Eq_tm s0)
-  | imp_tm s0 s1 =>
-      congr_imp_tm (compRenRen_tm xi_tm zeta_tm rho_tm Eq_tm s0)
-        (compRenRen_tm xi_tm zeta_tm rho_tm Eq_tm s1)
-  | forall_tm s0 =>
-      congr_forall_tm
-        (compRenRen_tm (upRen_tm_tm xi_tm) (upRen_tm_tm zeta_tm)
-           (upRen_tm_tm rho_tm) (up_ren_ren _ _ _ Eq_tm) s0)
-  | sort_tm s0 => congr_sort_tm (compRenRen_tm xi_tm zeta_tm rho_tm Eq_tm s0)
-  end.
-
-Lemma up_ren_subst_tm_tm (xi : nat -> nat) (tau : nat -> tm)
-  (theta : nat -> tm) (Eq : forall x, funcomp tau xi x = theta x) :
-  forall x, funcomp (up_tm_tm tau) (upRen_tm_tm xi) x = up_tm_tm theta x.
-Proof.
-exact (fun n =>
-       match n with
-       | S n' => ap (ren_tm shift) (Eq n')
-       | O => eq_refl
-       end).
-Qed.
-
-Fixpoint compRenSubst_tm (xi_tm : nat -> nat) (tau_tm : nat -> tm)
-(theta_tm : nat -> tm)
-(Eq_tm : forall x, funcomp tau_tm xi_tm x = theta_tm x) (s : tm) {struct s} :
-subst_tm tau_tm (ren_tm xi_tm s) = subst_tm theta_tm s :=
-  match s with
-  | var_tm s0 => Eq_tm s0
-  | lam_tm s0 =>
-      congr_lam_tm
-        (compRenSubst_tm (upRen_tm_tm xi_tm) (up_tm_tm tau_tm)
-           (up_tm_tm theta_tm) (up_ren_subst_tm_tm _ _ _ Eq_tm) s0)
-  | app_tm s0 s1 =>
-      congr_app_tm (compRenSubst_tm xi_tm tau_tm theta_tm Eq_tm s0)
-        (compRenSubst_tm xi_tm tau_tm theta_tm Eq_tm s1)
-  | z_tm => congr_z_tm
-  | s_tm s0 => congr_s_tm (compRenSubst_tm xi_tm tau_tm theta_tm Eq_tm s0)
-  | recN_tm s0 s1 s2 =>
-      congr_recN_tm (compRenSubst_tm xi_tm tau_tm theta_tm Eq_tm s0)
-        (compRenSubst_tm xi_tm tau_tm theta_tm Eq_tm s1)
-        (compRenSubst_tm xi_tm tau_tm theta_tm Eq_tm s2)
-  | tt_tm => congr_tt_tm
-  | ff_tm => congr_ff_tm
-  | recB_tm s0 s1 s2 =>
-      congr_recB_tm (compRenSubst_tm xi_tm tau_tm theta_tm Eq_tm s0)
-        (compRenSubst_tm xi_tm tau_tm theta_tm Eq_tm s1)
-        (compRenSubst_tm xi_tm tau_tm theta_tm Eq_tm s2)
-  | nil_tm => congr_nil_tm
-  | cons_tm s0 s1 =>
-      congr_cons_tm (compRenSubst_tm xi_tm tau_tm theta_tm Eq_tm s0)
-        (compRenSubst_tm xi_tm tau_tm theta_tm Eq_tm s1)
-  | recL_tm s0 s1 s2 =>
-      congr_recL_tm (compRenSubst_tm xi_tm tau_tm theta_tm Eq_tm s0)
-        (compRenSubst_tm xi_tm tau_tm theta_tm Eq_tm s1)
-        (compRenSubst_tm xi_tm tau_tm theta_tm Eq_tm s2)
-  | pair_tm s0 s1 =>
-      congr_pair_tm (compRenSubst_tm xi_tm tau_tm theta_tm Eq_tm s0)
-        (compRenSubst_tm xi_tm tau_tm theta_tm Eq_tm s1)
-  | pi1_tm s0 =>
-      congr_pi1_tm (compRenSubst_tm xi_tm tau_tm theta_tm Eq_tm s0)
-  | pi2_tm s0 =>
-      congr_pi2_tm (compRenSubst_tm xi_tm tau_tm theta_tm Eq_tm s0)
-  | imp_tm s0 s1 =>
-      congr_imp_tm (compRenSubst_tm xi_tm tau_tm theta_tm Eq_tm s0)
-        (compRenSubst_tm xi_tm tau_tm theta_tm Eq_tm s1)
-  | forall_tm s0 =>
-      congr_forall_tm
-        (compRenSubst_tm (upRen_tm_tm xi_tm) (up_tm_tm tau_tm)
-           (up_tm_tm theta_tm) (up_ren_subst_tm_tm _ _ _ Eq_tm) s0)
-  | sort_tm s0 =>
-      congr_sort_tm (compRenSubst_tm xi_tm tau_tm theta_tm Eq_tm s0)
-  end.
-
-Lemma up_subst_ren_tm_tm (sigma : nat -> tm) (zeta_tm : nat -> nat)
-  (theta : nat -> tm)
-  (Eq : forall x, funcomp (ren_tm zeta_tm) sigma x = theta x) :
-  forall x,
-  funcomp (ren_tm (upRen_tm_tm zeta_tm)) (up_tm_tm sigma) x =
-  up_tm_tm theta x.
-Proof.
-exact (fun n =>
-       match n with
-       | S n' =>
-           eq_trans
-             (compRenRen_tm shift (upRen_tm_tm zeta_tm)
-                (funcomp shift zeta_tm) (fun x => eq_refl) (sigma n'))
-             (eq_trans
-                (eq_sym
-                   (compRenRen_tm zeta_tm shift (funcomp shift zeta_tm)
-                      (fun x => eq_refl) (sigma n')))
-                (ap (ren_tm shift) (Eq n')))
-       | O => eq_refl
-       end).
-Qed.
-
-Fixpoint compSubstRen_tm (sigma_tm : nat -> tm) (zeta_tm : nat -> nat)
-(theta_tm : nat -> tm)
-(Eq_tm : forall x, funcomp (ren_tm zeta_tm) sigma_tm x = theta_tm x) 
-(s : tm) {struct s} :
-ren_tm zeta_tm (subst_tm sigma_tm s) = subst_tm theta_tm s :=
-  match s with
-  | var_tm s0 => Eq_tm s0
-  | lam_tm s0 =>
-      congr_lam_tm
-        (compSubstRen_tm (up_tm_tm sigma_tm) (upRen_tm_tm zeta_tm)
-           (up_tm_tm theta_tm) (up_subst_ren_tm_tm _ _ _ Eq_tm) s0)
-  | app_tm s0 s1 =>
-      congr_app_tm (compSubstRen_tm sigma_tm zeta_tm theta_tm Eq_tm s0)
-        (compSubstRen_tm sigma_tm zeta_tm theta_tm Eq_tm s1)
-  | z_tm => congr_z_tm
-  | s_tm s0 =>
-      congr_s_tm (compSubstRen_tm sigma_tm zeta_tm theta_tm Eq_tm s0)
-  | recN_tm s0 s1 s2 =>
-      congr_recN_tm (compSubstRen_tm sigma_tm zeta_tm theta_tm Eq_tm s0)
-        (compSubstRen_tm sigma_tm zeta_tm theta_tm Eq_tm s1)
-        (compSubstRen_tm sigma_tm zeta_tm theta_tm Eq_tm s2)
-  | tt_tm => congr_tt_tm
-  | ff_tm => congr_ff_tm
-  | recB_tm s0 s1 s2 =>
-      congr_recB_tm (compSubstRen_tm sigma_tm zeta_tm theta_tm Eq_tm s0)
-        (compSubstRen_tm sigma_tm zeta_tm theta_tm Eq_tm s1)
-        (compSubstRen_tm sigma_tm zeta_tm theta_tm Eq_tm s2)
-  | nil_tm => congr_nil_tm
-  | cons_tm s0 s1 =>
-      congr_cons_tm (compSubstRen_tm sigma_tm zeta_tm theta_tm Eq_tm s0)
-        (compSubstRen_tm sigma_tm zeta_tm theta_tm Eq_tm s1)
-  | recL_tm s0 s1 s2 =>
-      congr_recL_tm (compSubstRen_tm sigma_tm zeta_tm theta_tm Eq_tm s0)
-        (compSubstRen_tm sigma_tm zeta_tm theta_tm Eq_tm s1)
-        (compSubstRen_tm sigma_tm zeta_tm theta_tm Eq_tm s2)
-  | pair_tm s0 s1 =>
-      congr_pair_tm (compSubstRen_tm sigma_tm zeta_tm theta_tm Eq_tm s0)
-        (compSubstRen_tm sigma_tm zeta_tm theta_tm Eq_tm s1)
-  | pi1_tm s0 =>
-      congr_pi1_tm (compSubstRen_tm sigma_tm zeta_tm theta_tm Eq_tm s0)
-  | pi2_tm s0 =>
-      congr_pi2_tm (compSubstRen_tm sigma_tm zeta_tm theta_tm Eq_tm s0)
-  | imp_tm s0 s1 =>
-      congr_imp_tm (compSubstRen_tm sigma_tm zeta_tm theta_tm Eq_tm s0)
-        (compSubstRen_tm sigma_tm zeta_tm theta_tm Eq_tm s1)
-  | forall_tm s0 =>
-      congr_forall_tm
-        (compSubstRen_tm (up_tm_tm sigma_tm) (upRen_tm_tm zeta_tm)
-           (up_tm_tm theta_tm) (up_subst_ren_tm_tm _ _ _ Eq_tm) s0)
-  | sort_tm s0 =>
-      congr_sort_tm (compSubstRen_tm sigma_tm zeta_tm theta_tm Eq_tm s0)
-  end.
-
-Lemma up_subst_subst_tm_tm (sigma : nat -> tm) (tau_tm : nat -> tm)
-  (theta : nat -> tm)
-  (Eq : forall x, funcomp (subst_tm tau_tm) sigma x = theta x) :
-  forall x,
-  funcomp (subst_tm (up_tm_tm tau_tm)) (up_tm_tm sigma) x = up_tm_tm theta x.
-Proof.
-exact (fun n =>
-       match n with
-       | S n' =>
-           eq_trans
-             (compRenSubst_tm shift (up_tm_tm tau_tm)
-                (funcomp (up_tm_tm tau_tm) shift) (fun x => eq_refl)
-                (sigma n'))
-             (eq_trans
-                (eq_sym
-                   (compSubstRen_tm tau_tm shift
-                      (funcomp (ren_tm shift) tau_tm) (fun x => eq_refl)
-                      (sigma n'))) (ap (ren_tm shift) (Eq n')))
-       | O => eq_refl
-       end).
-Qed.
-
-Fixpoint compSubstSubst_tm (sigma_tm : nat -> tm) (tau_tm : nat -> tm)
-(theta_tm : nat -> tm)
-(Eq_tm : forall x, funcomp (subst_tm tau_tm) sigma_tm x = theta_tm x)
-(s : tm) {struct s} :
-subst_tm tau_tm (subst_tm sigma_tm s) = subst_tm theta_tm s :=
-  match s with
-  | var_tm s0 => Eq_tm s0
-  | lam_tm s0 =>
-      congr_lam_tm
-        (compSubstSubst_tm (up_tm_tm sigma_tm) (up_tm_tm tau_tm)
-           (up_tm_tm theta_tm) (up_subst_subst_tm_tm _ _ _ Eq_tm) s0)
-  | app_tm s0 s1 =>
-      congr_app_tm (compSubstSubst_tm sigma_tm tau_tm theta_tm Eq_tm s0)
-        (compSubstSubst_tm sigma_tm tau_tm theta_tm Eq_tm s1)
-  | z_tm => congr_z_tm
-  | s_tm s0 =>
-      congr_s_tm (compSubstSubst_tm sigma_tm tau_tm theta_tm Eq_tm s0)
-  | recN_tm s0 s1 s2 =>
-      congr_recN_tm (compSubstSubst_tm sigma_tm tau_tm theta_tm Eq_tm s0)
-        (compSubstSubst_tm sigma_tm tau_tm theta_tm Eq_tm s1)
-        (compSubstSubst_tm sigma_tm tau_tm theta_tm Eq_tm s2)
-  | tt_tm => congr_tt_tm
-  | ff_tm => congr_ff_tm
-  | recB_tm s0 s1 s2 =>
-      congr_recB_tm (compSubstSubst_tm sigma_tm tau_tm theta_tm Eq_tm s0)
-        (compSubstSubst_tm sigma_tm tau_tm theta_tm Eq_tm s1)
-        (compSubstSubst_tm sigma_tm tau_tm theta_tm Eq_tm s2)
-  | nil_tm => congr_nil_tm
-  | cons_tm s0 s1 =>
-      congr_cons_tm (compSubstSubst_tm sigma_tm tau_tm theta_tm Eq_tm s0)
-        (compSubstSubst_tm sigma_tm tau_tm theta_tm Eq_tm s1)
-  | recL_tm s0 s1 s2 =>
-      congr_recL_tm (compSubstSubst_tm sigma_tm tau_tm theta_tm Eq_tm s0)
-        (compSubstSubst_tm sigma_tm tau_tm theta_tm Eq_tm s1)
-        (compSubstSubst_tm sigma_tm tau_tm theta_tm Eq_tm s2)
-  | pair_tm s0 s1 =>
-      congr_pair_tm (compSubstSubst_tm sigma_tm tau_tm theta_tm Eq_tm s0)
-        (compSubstSubst_tm sigma_tm tau_tm theta_tm Eq_tm s1)
-  | pi1_tm s0 =>
-      congr_pi1_tm (compSubstSubst_tm sigma_tm tau_tm theta_tm Eq_tm s0)
-  | pi2_tm s0 =>
-      congr_pi2_tm (compSubstSubst_tm sigma_tm tau_tm theta_tm Eq_tm s0)
-  | imp_tm s0 s1 =>
-      congr_imp_tm (compSubstSubst_tm sigma_tm tau_tm theta_tm Eq_tm s0)
-        (compSubstSubst_tm sigma_tm tau_tm theta_tm Eq_tm s1)
-  | forall_tm s0 =>
-      congr_forall_tm
-        (compSubstSubst_tm (up_tm_tm sigma_tm) (up_tm_tm tau_tm)
-           (up_tm_tm theta_tm) (up_subst_subst_tm_tm _ _ _ Eq_tm) s0)
-  | sort_tm s0 =>
-      congr_sort_tm (compSubstSubst_tm sigma_tm tau_tm theta_tm Eq_tm s0)
-  end.
-
-Lemma renRen_tm (xi_tm : nat -> nat) (zeta_tm : nat -> nat) (s : tm) :
-  ren_tm zeta_tm (ren_tm xi_tm s) = ren_tm (funcomp zeta_tm xi_tm) s.
-Proof.
-exact (compRenRen_tm xi_tm zeta_tm _ (fun n => eq_refl) s).
-Qed.
-
-Lemma renRen'_tm_pointwise (xi_tm : nat -> nat) (zeta_tm : nat -> nat) :
-  pointwise_relation _ eq (funcomp (ren_tm zeta_tm) (ren_tm xi_tm))
-    (ren_tm (funcomp zeta_tm xi_tm)).
-Proof.
-exact (fun s => compRenRen_tm xi_tm zeta_tm _ (fun n => eq_refl) s).
-Qed.
-
-Lemma renSubst_tm (xi_tm : nat -> nat) (tau_tm : nat -> tm) (s : tm) :
-  subst_tm tau_tm (ren_tm xi_tm s) = subst_tm (funcomp tau_tm xi_tm) s.
-Proof.
-exact (compRenSubst_tm xi_tm tau_tm _ (fun n => eq_refl) s).
-Qed.
-
-Lemma renSubst_tm_pointwise (xi_tm : nat -> nat) (tau_tm : nat -> tm) :
-  pointwise_relation _ eq (funcomp (subst_tm tau_tm) (ren_tm xi_tm))
-    (subst_tm (funcomp tau_tm xi_tm)).
-Proof.
-exact (fun s => compRenSubst_tm xi_tm tau_tm _ (fun n => eq_refl) s).
-Qed.
-
-Lemma substRen_tm (sigma_tm : nat -> tm) (zeta_tm : nat -> nat) (s : tm) :
-  ren_tm zeta_tm (subst_tm sigma_tm s) =
-  subst_tm (funcomp (ren_tm zeta_tm) sigma_tm) s.
-Proof.
-exact (compSubstRen_tm sigma_tm zeta_tm _ (fun n => eq_refl) s).
-Qed.
-
-Lemma substRen_tm_pointwise (sigma_tm : nat -> tm) (zeta_tm : nat -> nat) :
-  pointwise_relation _ eq (funcomp (ren_tm zeta_tm) (subst_tm sigma_tm))
-    (subst_tm (funcomp (ren_tm zeta_tm) sigma_tm)).
-Proof.
-exact (fun s => compSubstRen_tm sigma_tm zeta_tm _ (fun n => eq_refl) s).
-Qed.
-
-Lemma substSubst_tm (sigma_tm : nat -> tm) (tau_tm : nat -> tm) (s : tm) :
-  subst_tm tau_tm (subst_tm sigma_tm s) =
-  subst_tm (funcomp (subst_tm tau_tm) sigma_tm) s.
-Proof.
-exact (compSubstSubst_tm sigma_tm tau_tm _ (fun n => eq_refl) s).
-Qed.
-
-Lemma substSubst_tm_pointwise (sigma_tm : nat -> tm) (tau_tm : nat -> tm) :
-  pointwise_relation _ eq (funcomp (subst_tm tau_tm) (subst_tm sigma_tm))
-    (subst_tm (funcomp (subst_tm tau_tm) sigma_tm)).
-Proof.
-exact (fun s => compSubstSubst_tm sigma_tm tau_tm _ (fun n => eq_refl) s).
-Qed.
-
-Lemma rinstInst_up_tm_tm (xi : nat -> nat) (sigma : nat -> tm)
-  (Eq : forall x, funcomp (var_tm) xi x = sigma x) :
-  forall x, funcomp (var_tm) (upRen_tm_tm xi) x = up_tm_tm sigma x.
-Proof.
-exact (fun n =>
-       match n with
-       | S n' => ap (ren_tm shift) (Eq n')
-       | O => eq_refl
-       end).
-Qed.
-
-Fixpoint rinst_inst_tm (xi_tm : nat -> nat) (sigma_tm : nat -> tm)
-(Eq_tm : forall x, funcomp (var_tm) xi_tm x = sigma_tm x) (s : tm) {struct s}
-   : ren_tm xi_tm s = subst_tm sigma_tm s :=
-  match s with
-  | var_tm s0 => Eq_tm s0
-  | lam_tm s0 =>
-      congr_lam_tm
-        (rinst_inst_tm (upRen_tm_tm xi_tm) (up_tm_tm sigma_tm)
-           (rinstInst_up_tm_tm _ _ Eq_tm) s0)
-  | app_tm s0 s1 =>
-      congr_app_tm (rinst_inst_tm xi_tm sigma_tm Eq_tm s0)
-        (rinst_inst_tm xi_tm sigma_tm Eq_tm s1)
-  | z_tm => congr_z_tm
-  | s_tm s0 => congr_s_tm (rinst_inst_tm xi_tm sigma_tm Eq_tm s0)
-  | recN_tm s0 s1 s2 =>
-      congr_recN_tm (rinst_inst_tm xi_tm sigma_tm Eq_tm s0)
-        (rinst_inst_tm xi_tm sigma_tm Eq_tm s1)
-        (rinst_inst_tm xi_tm sigma_tm Eq_tm s2)
-  | tt_tm => congr_tt_tm
-  | ff_tm => congr_ff_tm
-  | recB_tm s0 s1 s2 =>
-      congr_recB_tm (rinst_inst_tm xi_tm sigma_tm Eq_tm s0)
-        (rinst_inst_tm xi_tm sigma_tm Eq_tm s1)
-        (rinst_inst_tm xi_tm sigma_tm Eq_tm s2)
-  | nil_tm => congr_nil_tm
-  | cons_tm s0 s1 =>
-      congr_cons_tm (rinst_inst_tm xi_tm sigma_tm Eq_tm s0)
-        (rinst_inst_tm xi_tm sigma_tm Eq_tm s1)
-  | recL_tm s0 s1 s2 =>
-      congr_recL_tm (rinst_inst_tm xi_tm sigma_tm Eq_tm s0)
-        (rinst_inst_tm xi_tm sigma_tm Eq_tm s1)
-        (rinst_inst_tm xi_tm sigma_tm Eq_tm s2)
-  | pair_tm s0 s1 =>
-      congr_pair_tm (rinst_inst_tm xi_tm sigma_tm Eq_tm s0)
-        (rinst_inst_tm xi_tm sigma_tm Eq_tm s1)
-  | pi1_tm s0 => congr_pi1_tm (rinst_inst_tm xi_tm sigma_tm Eq_tm s0)
-  | pi2_tm s0 => congr_pi2_tm (rinst_inst_tm xi_tm sigma_tm Eq_tm s0)
-  | imp_tm s0 s1 =>
-      congr_imp_tm (rinst_inst_tm xi_tm sigma_tm Eq_tm s0)
-        (rinst_inst_tm xi_tm sigma_tm Eq_tm s1)
-  | forall_tm s0 =>
-      congr_forall_tm
-        (rinst_inst_tm (upRen_tm_tm xi_tm) (up_tm_tm sigma_tm)
-           (rinstInst_up_tm_tm _ _ Eq_tm) s0)
-  | sort_tm s0 => congr_sort_tm (rinst_inst_tm xi_tm sigma_tm Eq_tm s0)
-  end.
-
-Lemma rinstInst'_tm (xi_tm : nat -> nat) (s : tm) :
-  ren_tm xi_tm s = subst_tm (funcomp (var_tm) xi_tm) s.
-Proof.
-exact (rinst_inst_tm xi_tm _ (fun n => eq_refl) s).
-Qed.
-
-Lemma rinstInst'_tm_pointwise (xi_tm : nat -> nat) :
-  pointwise_relation _ eq (ren_tm xi_tm) (subst_tm (funcomp (var_tm) xi_tm)).
-Proof.
-exact (fun s => rinst_inst_tm xi_tm _ (fun n => eq_refl) s).
-Qed.
-
-Lemma instId'_tm (s : tm) : subst_tm (var_tm) s = s.
-Proof.
-exact (idSubst_tm (var_tm) (fun n => eq_refl) s).
-Qed.
-
-Lemma instId'_tm_pointwise : pointwise_relation _ eq (subst_tm (var_tm)) id.
-Proof.
-exact (fun s => idSubst_tm (var_tm) (fun n => eq_refl) s).
-Qed.
-
-Lemma rinstId'_tm (s : tm) : ren_tm id s = s.
-Proof.
-exact (eq_ind_r (fun t => t = s) (instId'_tm s) (rinstInst'_tm id s)).
-Qed.
-
-Lemma rinstId'_tm_pointwise : pointwise_relation _ eq (@ren_tm id) id.
-Proof.
-exact (fun s => eq_ind_r (fun t => t = s) (instId'_tm s) (rinstInst'_tm id s)).
-Qed.
-
-Lemma varL'_tm (sigma_tm : nat -> tm) (x : nat) :
-  subst_tm sigma_tm (var_tm x) = sigma_tm x.
-Proof.
-exact (eq_refl).
-Qed.
-
-Lemma varL'_tm_pointwise (sigma_tm : nat -> tm) :
-  pointwise_relation _ eq (funcomp (subst_tm sigma_tm) (var_tm)) sigma_tm.
-Proof.
-exact (fun x => eq_refl).
-Qed.
-
-Lemma varLRen'_tm (xi_tm : nat -> nat) (x : nat) :
-  ren_tm xi_tm (var_tm x) = var_tm (xi_tm x).
-Proof.
-exact (eq_refl).
-Qed.
-
-Lemma varLRen'_tm_pointwise (xi_tm : nat -> nat) :
-  pointwise_relation _ eq (funcomp (ren_tm xi_tm) (var_tm))
-    (funcomp (var_tm) xi_tm).
-Proof.
-exact (fun x => eq_refl).
-Qed.
-
-Class Up_tm X Y :=
+  Inductive st : Type :=
+  | nat_st : st
+  | bool_st : st
+  | list_st : st -> st
+  | prop_st : st
+  | to_st : st -> st -> st
+  | prod_st : st -> st -> st.
+
+  Notation ℕₛ := nat_st.
+  Notation 𝔹ₛ := bool_st.
+  Notation 𝕃ₛ := list_st.
+  Notation ℙₛ := prop_st.
+  Notation "s →ₛ s'" := (to_st s s') (at level 86, right associativity).
+  Notation "s ×ₛ s'" := (prod_st s s') (at level 86, right associativity).
+
+  Lemma congr_nat_st : nat_st = nat_st.
+  Proof.
+    exact (eq_refl).
+  Qed.
+
+  Lemma congr_bool_st : bool_st = bool_st.
+  Proof.
+    exact (eq_refl).
+  Qed.
+
+  Lemma congr_list_st {s0 : st} {t0 : st} (H0 : s0 = t0) :
+    list_st s0 = list_st t0.
+  Proof.
+    exact (eq_trans eq_refl (ap (fun x => list_st x) H0)).
+  Qed.
+
+  Lemma congr_prop_st : prop_st = prop_st.
+  Proof.
+    exact (eq_refl).
+  Qed.
+
+  Lemma congr_to_st {s0 : st} {s1 : st} {t0 : st} {t1 : st} (H0 : s0 = t0)
+    (H1 : s1 = t1) : to_st s0 s1 = to_st t0 t1.
+  Proof.
+    exact (eq_trans (eq_trans eq_refl (ap (fun x => to_st x s1) H0))
+             (ap (fun x => to_st t0 x) H1)).
+  Qed.
+
+  Lemma congr_prod_st {s0 : st} {s1 : st} {t0 : st} {t1 : st} (H0 : s0 = t0)
+    (H1 : s1 = t1) : prod_st s0 s1 = prod_st t0 t1.
+  Proof.
+    exact (eq_trans (eq_trans eq_refl (ap (fun x => prod_st x s1) H0))
+             (ap (fun x => prod_st t0 x) H1)).
+  Qed.
+
+  Inductive tm (n_tm : nat) : Type :=
+  | var_tm : fin n_tm -> tm n_tm
+  | lam_tm : tm (S n_tm) -> tm n_tm
+  | app_tm : tm n_tm -> tm n_tm -> tm n_tm
+  | z_tm : tm n_tm
+  | s_tm : tm n_tm -> tm n_tm
+  | recN_tm : tm n_tm -> tm n_tm -> tm n_tm -> tm n_tm
+  | tt_tm : tm n_tm
+  | ff_tm : tm n_tm
+  | recB_tm : tm n_tm -> tm n_tm -> tm n_tm -> tm n_tm
+  | nil_tm : tm n_tm
+  | cons_tm : tm n_tm -> tm n_tm -> tm n_tm
+  | recL_tm : tm n_tm -> tm n_tm -> tm n_tm -> tm n_tm
+  | pair_tm : tm n_tm -> tm n_tm -> tm n_tm
+  | pi1_tm : tm n_tm -> tm n_tm
+  | pi2_tm : tm n_tm -> tm n_tm
+  | imp_tm : tm n_tm -> tm n_tm -> tm n_tm
+  | forall_tm : tm (S n_tm) -> tm n_tm
+  | sort_tm : st -> tm n_tm -> tm n_tm.
+  
+  Notation "⟦ n ⟧ₛ" := (var_tm _ n).
+  Notation ƛ := (lam_tm _).
+  Notation "t @ₛ u" := (app_tm _ t u) (at level 88, left associativity).
+  Notation Zₛ := (z_tm _).
+  Notation Sₛ := (s_tm _).
+  Notation recℕₛ := (recN_tm _).
+  Notation ttₛ := (tt_tm _).
+  Notation ffₛ := (ff_tm _).
+  Notation rec𝔹ₛ := (recB_tm _).
+  Notation "[]ₛ" := (nil_tm _).
+  Notation "t ::ₛ u" := (cons_tm _ t u) (at level 86, right associativity).
+  Notation rec𝕃ₛ := (recL_tm _).
+  Notation "⟨ t , u ⟩ₛ" := (pair_tm _ t u).
+  Notation "π¹ₛ" := (pi1_tm _).
+  Notation "π²ₛ" := (pi2_tm _).
+  Notation "φ ⇒ₛ ψ" := (imp_tm _ φ ψ) (at level 89, right associativity).
+  Notation "∀ₛ" := (forall_tm _).
+  Notation 𝕊 := (sort_tm _).
+
+  Lemma congr_lam_tm {m_tm : nat} {s0 : tm (S m_tm)} {t0 : tm (S m_tm)}
+    (H0 : s0 = t0) : lam_tm m_tm s0 = lam_tm m_tm t0.
+  Proof.
+    exact (eq_trans eq_refl (ap (fun x => lam_tm m_tm x) H0)).
+  Qed.
+
+  Lemma congr_app_tm {m_tm : nat} {s0 : tm m_tm} {s1 : tm m_tm} {t0 : tm m_tm}
+    {t1 : tm m_tm} (H0 : s0 = t0) (H1 : s1 = t1) :
+    app_tm m_tm s0 s1 = app_tm m_tm t0 t1.
+  Proof.
+    exact (eq_trans (eq_trans eq_refl (ap (fun x => app_tm m_tm x s1) H0))
+             (ap (fun x => app_tm m_tm t0 x) H1)).
+  Qed.
+
+  Lemma congr_z_tm {m_tm : nat} : z_tm m_tm = z_tm m_tm.
+  Proof.
+    exact (eq_refl).
+  Qed.
+
+  Lemma congr_s_tm {m_tm : nat} {s0 : tm m_tm} {t0 : tm m_tm} (H0 : s0 = t0) :
+    s_tm m_tm s0 = s_tm m_tm t0.
+  Proof.
+    exact (eq_trans eq_refl (ap (fun x => s_tm m_tm x) H0)).
+  Qed.
+
+  Lemma congr_recN_tm {m_tm : nat} {s0 : tm m_tm} {s1 : tm m_tm} {s2 : tm m_tm}
+    {t0 : tm m_tm} {t1 : tm m_tm} {t2 : tm m_tm} (H0 : s0 = t0) (H1 : s1 = t1)
+    (H2 : s2 = t2) : recN_tm m_tm s0 s1 s2 = recN_tm m_tm t0 t1 t2.
+  Proof.
+    exact (eq_trans
+             (eq_trans (eq_trans eq_refl (ap (fun x => recN_tm m_tm x s1 s2) H0))
+                (ap (fun x => recN_tm m_tm t0 x s2) H1))
+             (ap (fun x => recN_tm m_tm t0 t1 x) H2)).
+  Qed.
+
+  Lemma congr_tt_tm {m_tm : nat} : tt_tm m_tm = tt_tm m_tm.
+  Proof.
+    exact (eq_refl).
+  Qed.
+
+  Lemma congr_ff_tm {m_tm : nat} : ff_tm m_tm = ff_tm m_tm.
+  Proof.
+    exact (eq_refl).
+  Qed.
+
+  Lemma congr_recB_tm {m_tm : nat} {s0 : tm m_tm} {s1 : tm m_tm} {s2 : tm m_tm}
+    {t0 : tm m_tm} {t1 : tm m_tm} {t2 : tm m_tm} (H0 : s0 = t0) (H1 : s1 = t1)
+    (H2 : s2 = t2) : recB_tm m_tm s0 s1 s2 = recB_tm m_tm t0 t1 t2.
+  Proof.
+    exact (eq_trans
+             (eq_trans (eq_trans eq_refl (ap (fun x => recB_tm m_tm x s1 s2) H0))
+                (ap (fun x => recB_tm m_tm t0 x s2) H1))
+             (ap (fun x => recB_tm m_tm t0 t1 x) H2)).
+  Qed.
+
+  Lemma congr_nil_tm {m_tm : nat} : nil_tm m_tm = nil_tm m_tm.
+  Proof.
+    exact (eq_refl).
+  Qed.
+
+  Lemma congr_cons_tm {m_tm : nat} {s0 : tm m_tm} {s1 : tm m_tm} {t0 : tm m_tm}
+    {t1 : tm m_tm} (H0 : s0 = t0) (H1 : s1 = t1) :
+    cons_tm m_tm s0 s1 = cons_tm m_tm t0 t1.
+  Proof.
+    exact (eq_trans (eq_trans eq_refl (ap (fun x => cons_tm m_tm x s1) H0))
+             (ap (fun x => cons_tm m_tm t0 x) H1)).
+  Qed.
+
+  Lemma congr_recL_tm {m_tm : nat} {s0 : tm m_tm} {s1 : tm m_tm} {s2 : tm m_tm}
+    {t0 : tm m_tm} {t1 : tm m_tm} {t2 : tm m_tm} (H0 : s0 = t0) (H1 : s1 = t1)
+    (H2 : s2 = t2) : recL_tm m_tm s0 s1 s2 = recL_tm m_tm t0 t1 t2.
+  Proof.
+    exact (eq_trans
+             (eq_trans (eq_trans eq_refl (ap (fun x => recL_tm m_tm x s1 s2) H0))
+                (ap (fun x => recL_tm m_tm t0 x s2) H1))
+             (ap (fun x => recL_tm m_tm t0 t1 x) H2)).
+  Qed.
+
+  Lemma congr_pair_tm {m_tm : nat} {s0 : tm m_tm} {s1 : tm m_tm} {t0 : tm m_tm}
+    {t1 : tm m_tm} (H0 : s0 = t0) (H1 : s1 = t1) :
+    pair_tm m_tm s0 s1 = pair_tm m_tm t0 t1.
+  Proof.
+    exact (eq_trans (eq_trans eq_refl (ap (fun x => pair_tm m_tm x s1) H0))
+             (ap (fun x => pair_tm m_tm t0 x) H1)).
+  Qed.
+
+  Lemma congr_pi1_tm {m_tm : nat} {s0 : tm m_tm} {t0 : tm m_tm} (H0 : s0 = t0)
+    : pi1_tm m_tm s0 = pi1_tm m_tm t0.
+  Proof.
+    exact (eq_trans eq_refl (ap (fun x => pi1_tm m_tm x) H0)).
+  Qed.
+
+  Lemma congr_pi2_tm {m_tm : nat} {s0 : tm m_tm} {t0 : tm m_tm} (H0 : s0 = t0)
+    : pi2_tm m_tm s0 = pi2_tm m_tm t0.
+  Proof.
+    exact (eq_trans eq_refl (ap (fun x => pi2_tm m_tm x) H0)).
+  Qed.
+
+  Lemma congr_imp_tm {m_tm : nat} {s0 : tm m_tm} {s1 : tm m_tm} {t0 : tm m_tm}
+    {t1 : tm m_tm} (H0 : s0 = t0) (H1 : s1 = t1) :
+    imp_tm m_tm s0 s1 = imp_tm m_tm t0 t1.
+  Proof.
+    exact (eq_trans (eq_trans eq_refl (ap (fun x => imp_tm m_tm x s1) H0))
+             (ap (fun x => imp_tm m_tm t0 x) H1)).
+  Qed.
+
+  Lemma congr_forall_tm {m_tm : nat} {s0 : tm (S m_tm)} {t0 : tm (S m_tm)}
+    (H0 : s0 = t0) : forall_tm m_tm s0 = forall_tm m_tm t0.
+  Proof.
+    exact (eq_trans eq_refl (ap (fun x => forall_tm m_tm x) H0)).
+  Qed.
+
+  Lemma congr_sort_tm {m_tm : nat} {s0 : st} {s1 : tm m_tm} {t0 : st}
+    {t1 : tm m_tm} (H0 : s0 = t0) (H1 : s1 = t1) :
+    sort_tm m_tm s0 s1 = sort_tm m_tm t0 t1.
+  Proof.
+    exact (eq_trans (eq_trans eq_refl (ap (fun x => sort_tm m_tm x s1) H0))
+             (ap (fun x => sort_tm m_tm t0 x) H1)).
+  Qed.
+
+  Lemma upRen_tm_tm {m : nat} {n : nat} (xi : fin m -> fin n) :
+    fin (S m) -> fin (S n).
+  Proof.
+    exact (up_ren xi).
+  Defined.
+
+  Lemma upRen_list_tm_tm (p : nat) {m : nat} {n : nat} (xi : fin m -> fin n) :
+    fin (plus p m) -> fin (plus p n).
+  Proof.
+    exact (upRen_p p xi).
+  Defined.
+
+  Fixpoint ren_tm {m_tm : nat} {n_tm : nat} (xi_tm : fin m_tm -> fin n_tm)
+    (s : tm m_tm) {struct s} : tm n_tm :=
+    match s with
+    | var_tm _ s0 => var_tm n_tm (xi_tm s0)
+    | lam_tm _ s0 => lam_tm n_tm (ren_tm (upRen_tm_tm xi_tm) s0)
+    | app_tm _ s0 s1 => app_tm n_tm (ren_tm xi_tm s0) (ren_tm xi_tm s1)
+    | z_tm _ => z_tm n_tm
+    | s_tm _ s0 => s_tm n_tm (ren_tm xi_tm s0)
+    | recN_tm _ s0 s1 s2 =>
+        recN_tm n_tm (ren_tm xi_tm s0) (ren_tm xi_tm s1) (ren_tm xi_tm s2)
+    | tt_tm _ => tt_tm n_tm
+    | ff_tm _ => ff_tm n_tm
+    | recB_tm _ s0 s1 s2 =>
+        recB_tm n_tm (ren_tm xi_tm s0) (ren_tm xi_tm s1) (ren_tm xi_tm s2)
+    | nil_tm _ => nil_tm n_tm
+    | cons_tm _ s0 s1 => cons_tm n_tm (ren_tm xi_tm s0) (ren_tm xi_tm s1)
+    | recL_tm _ s0 s1 s2 =>
+        recL_tm n_tm (ren_tm xi_tm s0) (ren_tm xi_tm s1) (ren_tm xi_tm s2)
+    | pair_tm _ s0 s1 => pair_tm n_tm (ren_tm xi_tm s0) (ren_tm xi_tm s1)
+    | pi1_tm _ s0 => pi1_tm n_tm (ren_tm xi_tm s0)
+    | pi2_tm _ s0 => pi2_tm n_tm (ren_tm xi_tm s0)
+    | imp_tm _ s0 s1 => imp_tm n_tm (ren_tm xi_tm s0) (ren_tm xi_tm s1)
+    | forall_tm _ s0 => forall_tm n_tm (ren_tm (upRen_tm_tm xi_tm) s0)
+    | sort_tm _ s0 s1 => sort_tm n_tm s0 (ren_tm xi_tm s1)
+    end.
+
+  Lemma up_tm_tm {m : nat} {n_tm : nat} (sigma : fin m -> tm n_tm) :
+    fin (S m) -> tm (S n_tm).
+  Proof.
+    exact (scons (var_tm (S n_tm) var_zero) (funcomp (ren_tm shift) sigma)).
+  Defined.
+
+  Lemma up_list_tm_tm (p : nat) {m : nat} {n_tm : nat}
+    (sigma : fin m -> tm n_tm) : fin (plus p m) -> tm (plus p n_tm).
+  Proof.
+    exact (scons_p p (funcomp (var_tm (plus p n_tm)) (zero_p p))
+             (funcomp (ren_tm (shift_p p)) sigma)).
+  Defined.
+
+  Fixpoint subst_tm {m_tm : nat} {n_tm : nat} (sigma_tm : fin m_tm -> tm n_tm)
+    (s : tm m_tm) {struct s} : tm n_tm :=
+    match s with
+    | var_tm _ s0 => sigma_tm s0
+    | lam_tm _ s0 => lam_tm n_tm (subst_tm (up_tm_tm sigma_tm) s0)
+    | app_tm _ s0 s1 =>
+        app_tm n_tm (subst_tm sigma_tm s0) (subst_tm sigma_tm s1)
+    | z_tm _ => z_tm n_tm
+    | s_tm _ s0 => s_tm n_tm (subst_tm sigma_tm s0)
+    | recN_tm _ s0 s1 s2 =>
+        recN_tm n_tm (subst_tm sigma_tm s0) (subst_tm sigma_tm s1)
+          (subst_tm sigma_tm s2)
+    | tt_tm _ => tt_tm n_tm
+    | ff_tm _ => ff_tm n_tm
+    | recB_tm _ s0 s1 s2 =>
+        recB_tm n_tm (subst_tm sigma_tm s0) (subst_tm sigma_tm s1)
+          (subst_tm sigma_tm s2)
+    | nil_tm _ => nil_tm n_tm
+    | cons_tm _ s0 s1 =>
+        cons_tm n_tm (subst_tm sigma_tm s0) (subst_tm sigma_tm s1)
+    | recL_tm _ s0 s1 s2 =>
+        recL_tm n_tm (subst_tm sigma_tm s0) (subst_tm sigma_tm s1)
+          (subst_tm sigma_tm s2)
+    | pair_tm _ s0 s1 =>
+        pair_tm n_tm (subst_tm sigma_tm s0) (subst_tm sigma_tm s1)
+    | pi1_tm _ s0 => pi1_tm n_tm (subst_tm sigma_tm s0)
+    | pi2_tm _ s0 => pi2_tm n_tm (subst_tm sigma_tm s0)
+    | imp_tm _ s0 s1 =>
+        imp_tm n_tm (subst_tm sigma_tm s0) (subst_tm sigma_tm s1)
+    | forall_tm _ s0 => forall_tm n_tm (subst_tm (up_tm_tm sigma_tm) s0)
+    | sort_tm _ s0 s1 => sort_tm n_tm s0 (subst_tm sigma_tm s1)
+    end.
+
+  Lemma upId_tm_tm {m_tm : nat} (sigma : fin m_tm -> tm m_tm)
+    (Eq : forall x, sigma x = var_tm m_tm x) :
+    forall x, up_tm_tm sigma x = var_tm (S m_tm) x.
+  Proof.
+    exact (fun n =>
+             match n with
+             | Some fin_n => ap (ren_tm shift) (Eq fin_n)
+             | None => eq_refl
+             end).
+  Qed.
+
+  Lemma upId_list_tm_tm {p : nat} {m_tm : nat} (sigma : fin m_tm -> tm m_tm)
+    (Eq : forall x, sigma x = var_tm m_tm x) :
+    forall x, up_list_tm_tm p sigma x = var_tm (plus p m_tm) x.
+  Proof.
+    exact (fun n =>
+             scons_p_eta (var_tm (plus p m_tm))
+               (fun n => ap (ren_tm (shift_p p)) (Eq n)) (fun n => eq_refl)).
+  Qed.
+
+  Fixpoint idSubst_tm {m_tm : nat} (sigma_tm : fin m_tm -> tm m_tm)
+    (Eq_tm : forall x, sigma_tm x = var_tm m_tm x) (s : tm m_tm) {struct s} :
+    subst_tm sigma_tm s = s :=
+    match s with
+    | var_tm _ s0 => Eq_tm s0
+    | lam_tm _ s0 =>
+        congr_lam_tm (idSubst_tm (up_tm_tm sigma_tm) (upId_tm_tm _ Eq_tm) s0)
+    | app_tm _ s0 s1 =>
+        congr_app_tm (idSubst_tm sigma_tm Eq_tm s0)
+          (idSubst_tm sigma_tm Eq_tm s1)
+    | z_tm _ => congr_z_tm
+    | s_tm _ s0 => congr_s_tm (idSubst_tm sigma_tm Eq_tm s0)
+    | recN_tm _ s0 s1 s2 =>
+        congr_recN_tm (idSubst_tm sigma_tm Eq_tm s0)
+          (idSubst_tm sigma_tm Eq_tm s1) (idSubst_tm sigma_tm Eq_tm s2)
+    | tt_tm _ => congr_tt_tm
+    | ff_tm _ => congr_ff_tm
+    | recB_tm _ s0 s1 s2 =>
+        congr_recB_tm (idSubst_tm sigma_tm Eq_tm s0)
+          (idSubst_tm sigma_tm Eq_tm s1) (idSubst_tm sigma_tm Eq_tm s2)
+    | nil_tm _ => congr_nil_tm
+    | cons_tm _ s0 s1 =>
+        congr_cons_tm (idSubst_tm sigma_tm Eq_tm s0)
+          (idSubst_tm sigma_tm Eq_tm s1)
+    | recL_tm _ s0 s1 s2 =>
+        congr_recL_tm (idSubst_tm sigma_tm Eq_tm s0)
+          (idSubst_tm sigma_tm Eq_tm s1) (idSubst_tm sigma_tm Eq_tm s2)
+    | pair_tm _ s0 s1 =>
+        congr_pair_tm (idSubst_tm sigma_tm Eq_tm s0)
+          (idSubst_tm sigma_tm Eq_tm s1)
+    | pi1_tm _ s0 => congr_pi1_tm (idSubst_tm sigma_tm Eq_tm s0)
+    | pi2_tm _ s0 => congr_pi2_tm (idSubst_tm sigma_tm Eq_tm s0)
+    | imp_tm _ s0 s1 =>
+        congr_imp_tm (idSubst_tm sigma_tm Eq_tm s0)
+          (idSubst_tm sigma_tm Eq_tm s1)
+    | forall_tm _ s0 =>
+        congr_forall_tm
+          (idSubst_tm (up_tm_tm sigma_tm) (upId_tm_tm _ Eq_tm) s0)
+    | sort_tm _ s0 s1 =>
+        congr_sort_tm (eq_refl s0) (idSubst_tm sigma_tm Eq_tm s1)
+    end.
+
+  Lemma upExtRen_tm_tm {m : nat} {n : nat} (xi : fin m -> fin n)
+    (zeta : fin m -> fin n) (Eq : forall x, xi x = zeta x) :
+    forall x, upRen_tm_tm xi x = upRen_tm_tm zeta x.
+  Proof.
+    exact (fun n =>
+             match n with
+             | Some fin_n => ap shift (Eq fin_n)
+             | None => eq_refl
+             end).
+  Qed.
+
+  Lemma upExtRen_list_tm_tm {p : nat} {m : nat} {n : nat} (xi : fin m -> fin n)
+    (zeta : fin m -> fin n) (Eq : forall x, xi x = zeta x) :
+    forall x, upRen_list_tm_tm p xi x = upRen_list_tm_tm p zeta x.
+  Proof.
+    exact (fun n =>
+             scons_p_congr (fun n => eq_refl) (fun n => ap (shift_p p) (Eq n))).
+  Qed.
+
+  Fixpoint extRen_tm {m_tm : nat} {n_tm : nat} (xi_tm : fin m_tm -> fin n_tm)
+    (zeta_tm : fin m_tm -> fin n_tm) (Eq_tm : forall x, xi_tm x = zeta_tm x)
+    (s : tm m_tm) {struct s} : ren_tm xi_tm s = ren_tm zeta_tm s :=
+    match s with
+    | var_tm _ s0 => ap (var_tm n_tm) (Eq_tm s0)
+    | lam_tm _ s0 =>
+        congr_lam_tm
+          (extRen_tm (upRen_tm_tm xi_tm) (upRen_tm_tm zeta_tm)
+             (upExtRen_tm_tm _ _ Eq_tm) s0)
+    | app_tm _ s0 s1 =>
+        congr_app_tm (extRen_tm xi_tm zeta_tm Eq_tm s0)
+          (extRen_tm xi_tm zeta_tm Eq_tm s1)
+    | z_tm _ => congr_z_tm
+    | s_tm _ s0 => congr_s_tm (extRen_tm xi_tm zeta_tm Eq_tm s0)
+    | recN_tm _ s0 s1 s2 =>
+        congr_recN_tm (extRen_tm xi_tm zeta_tm Eq_tm s0)
+          (extRen_tm xi_tm zeta_tm Eq_tm s1) (extRen_tm xi_tm zeta_tm Eq_tm s2)
+    | tt_tm _ => congr_tt_tm
+    | ff_tm _ => congr_ff_tm
+    | recB_tm _ s0 s1 s2 =>
+        congr_recB_tm (extRen_tm xi_tm zeta_tm Eq_tm s0)
+          (extRen_tm xi_tm zeta_tm Eq_tm s1) (extRen_tm xi_tm zeta_tm Eq_tm s2)
+    | nil_tm _ => congr_nil_tm
+    | cons_tm _ s0 s1 =>
+        congr_cons_tm (extRen_tm xi_tm zeta_tm Eq_tm s0)
+          (extRen_tm xi_tm zeta_tm Eq_tm s1)
+    | recL_tm _ s0 s1 s2 =>
+        congr_recL_tm (extRen_tm xi_tm zeta_tm Eq_tm s0)
+          (extRen_tm xi_tm zeta_tm Eq_tm s1) (extRen_tm xi_tm zeta_tm Eq_tm s2)
+    | pair_tm _ s0 s1 =>
+        congr_pair_tm (extRen_tm xi_tm zeta_tm Eq_tm s0)
+          (extRen_tm xi_tm zeta_tm Eq_tm s1)
+    | pi1_tm _ s0 => congr_pi1_tm (extRen_tm xi_tm zeta_tm Eq_tm s0)
+    | pi2_tm _ s0 => congr_pi2_tm (extRen_tm xi_tm zeta_tm Eq_tm s0)
+    | imp_tm _ s0 s1 =>
+        congr_imp_tm (extRen_tm xi_tm zeta_tm Eq_tm s0)
+          (extRen_tm xi_tm zeta_tm Eq_tm s1)
+    | forall_tm _ s0 =>
+        congr_forall_tm
+          (extRen_tm (upRen_tm_tm xi_tm) (upRen_tm_tm zeta_tm)
+             (upExtRen_tm_tm _ _ Eq_tm) s0)
+    | sort_tm _ s0 s1 =>
+        congr_sort_tm (eq_refl s0) (extRen_tm xi_tm zeta_tm Eq_tm s1)
+    end.
+
+  Lemma upExt_tm_tm {m : nat} {n_tm : nat} (sigma : fin m -> tm n_tm)
+    (tau : fin m -> tm n_tm) (Eq : forall x, sigma x = tau x) :
+    forall x, up_tm_tm sigma x = up_tm_tm tau x.
+  Proof.
+    exact (fun n =>
+             match n with
+             | Some fin_n => ap (ren_tm shift) (Eq fin_n)
+             | None => eq_refl
+             end).
+  Qed.
+
+  Lemma upExt_list_tm_tm {p : nat} {m : nat} {n_tm : nat}
+    (sigma : fin m -> tm n_tm) (tau : fin m -> tm n_tm)
+    (Eq : forall x, sigma x = tau x) :
+    forall x, up_list_tm_tm p sigma x = up_list_tm_tm p tau x.
+  Proof.
+    exact (fun n =>
+             scons_p_congr (fun n => eq_refl)
+               (fun n => ap (ren_tm (shift_p p)) (Eq n))).
+  Qed.
+
+  Fixpoint ext_tm {m_tm : nat} {n_tm : nat} (sigma_tm : fin m_tm -> tm n_tm)
+    (tau_tm : fin m_tm -> tm n_tm) (Eq_tm : forall x, sigma_tm x = tau_tm x)
+    (s : tm m_tm) {struct s} : subst_tm sigma_tm s = subst_tm tau_tm s :=
+    match s with
+    | var_tm _ s0 => Eq_tm s0
+    | lam_tm _ s0 =>
+        congr_lam_tm
+          (ext_tm (up_tm_tm sigma_tm) (up_tm_tm tau_tm) (upExt_tm_tm _ _ Eq_tm)
+             s0)
+    | app_tm _ s0 s1 =>
+        congr_app_tm (ext_tm sigma_tm tau_tm Eq_tm s0)
+          (ext_tm sigma_tm tau_tm Eq_tm s1)
+    | z_tm _ => congr_z_tm
+    | s_tm _ s0 => congr_s_tm (ext_tm sigma_tm tau_tm Eq_tm s0)
+    | recN_tm _ s0 s1 s2 =>
+        congr_recN_tm (ext_tm sigma_tm tau_tm Eq_tm s0)
+          (ext_tm sigma_tm tau_tm Eq_tm s1) (ext_tm sigma_tm tau_tm Eq_tm s2)
+    | tt_tm _ => congr_tt_tm
+    | ff_tm _ => congr_ff_tm
+    | recB_tm _ s0 s1 s2 =>
+        congr_recB_tm (ext_tm sigma_tm tau_tm Eq_tm s0)
+          (ext_tm sigma_tm tau_tm Eq_tm s1) (ext_tm sigma_tm tau_tm Eq_tm s2)
+    | nil_tm _ => congr_nil_tm
+    | cons_tm _ s0 s1 =>
+        congr_cons_tm (ext_tm sigma_tm tau_tm Eq_tm s0)
+          (ext_tm sigma_tm tau_tm Eq_tm s1)
+    | recL_tm _ s0 s1 s2 =>
+        congr_recL_tm (ext_tm sigma_tm tau_tm Eq_tm s0)
+          (ext_tm sigma_tm tau_tm Eq_tm s1) (ext_tm sigma_tm tau_tm Eq_tm s2)
+    | pair_tm _ s0 s1 =>
+        congr_pair_tm (ext_tm sigma_tm tau_tm Eq_tm s0)
+          (ext_tm sigma_tm tau_tm Eq_tm s1)
+    | pi1_tm _ s0 => congr_pi1_tm (ext_tm sigma_tm tau_tm Eq_tm s0)
+    | pi2_tm _ s0 => congr_pi2_tm (ext_tm sigma_tm tau_tm Eq_tm s0)
+    | imp_tm _ s0 s1 =>
+        congr_imp_tm (ext_tm sigma_tm tau_tm Eq_tm s0)
+          (ext_tm sigma_tm tau_tm Eq_tm s1)
+    | forall_tm _ s0 =>
+        congr_forall_tm
+          (ext_tm (up_tm_tm sigma_tm) (up_tm_tm tau_tm) (upExt_tm_tm _ _ Eq_tm)
+             s0)
+    | sort_tm _ s0 s1 =>
+        congr_sort_tm (eq_refl s0) (ext_tm sigma_tm tau_tm Eq_tm s1)
+    end.
+
+  Lemma up_ren_ren_tm_tm {k : nat} {l : nat} {m : nat} (xi : fin k -> fin l)
+    (zeta : fin l -> fin m) (rho : fin k -> fin m)
+    (Eq : forall x, funcomp zeta xi x = rho x) :
+    forall x, funcomp (upRen_tm_tm zeta) (upRen_tm_tm xi) x = upRen_tm_tm rho x.
+  Proof.
+    exact (up_ren_ren xi zeta rho Eq).
+  Qed.
+
+  Lemma up_ren_ren_list_tm_tm {p : nat} {k : nat} {l : nat} {m : nat}
+    (xi : fin k -> fin l) (zeta : fin l -> fin m) (rho : fin k -> fin m)
+    (Eq : forall x, funcomp zeta xi x = rho x) :
+    forall x,
+      funcomp (upRen_list_tm_tm p zeta) (upRen_list_tm_tm p xi) x =
+        upRen_list_tm_tm p rho x.
+  Proof.
+    exact (up_ren_ren_p Eq).
+  Qed.
+
+  Fixpoint compRenRen_tm {k_tm : nat} {l_tm : nat} {m_tm : nat}
+    (xi_tm : fin m_tm -> fin k_tm) (zeta_tm : fin k_tm -> fin l_tm)
+    (rho_tm : fin m_tm -> fin l_tm)
+    (Eq_tm : forall x, funcomp zeta_tm xi_tm x = rho_tm x) (s : tm m_tm) {struct
+                                                                            s} : ren_tm zeta_tm (ren_tm xi_tm s) = ren_tm rho_tm s :=
+    match s with
+    | var_tm _ s0 => ap (var_tm l_tm) (Eq_tm s0)
+    | lam_tm _ s0 =>
+        congr_lam_tm
+          (compRenRen_tm (upRen_tm_tm xi_tm) (upRen_tm_tm zeta_tm)
+             (upRen_tm_tm rho_tm) (up_ren_ren _ _ _ Eq_tm) s0)
+    | app_tm _ s0 s1 =>
+        congr_app_tm (compRenRen_tm xi_tm zeta_tm rho_tm Eq_tm s0)
+          (compRenRen_tm xi_tm zeta_tm rho_tm Eq_tm s1)
+    | z_tm _ => congr_z_tm
+    | s_tm _ s0 => congr_s_tm (compRenRen_tm xi_tm zeta_tm rho_tm Eq_tm s0)
+    | recN_tm _ s0 s1 s2 =>
+        congr_recN_tm (compRenRen_tm xi_tm zeta_tm rho_tm Eq_tm s0)
+          (compRenRen_tm xi_tm zeta_tm rho_tm Eq_tm s1)
+          (compRenRen_tm xi_tm zeta_tm rho_tm Eq_tm s2)
+    | tt_tm _ => congr_tt_tm
+    | ff_tm _ => congr_ff_tm
+    | recB_tm _ s0 s1 s2 =>
+        congr_recB_tm (compRenRen_tm xi_tm zeta_tm rho_tm Eq_tm s0)
+          (compRenRen_tm xi_tm zeta_tm rho_tm Eq_tm s1)
+          (compRenRen_tm xi_tm zeta_tm rho_tm Eq_tm s2)
+    | nil_tm _ => congr_nil_tm
+    | cons_tm _ s0 s1 =>
+        congr_cons_tm (compRenRen_tm xi_tm zeta_tm rho_tm Eq_tm s0)
+          (compRenRen_tm xi_tm zeta_tm rho_tm Eq_tm s1)
+    | recL_tm _ s0 s1 s2 =>
+        congr_recL_tm (compRenRen_tm xi_tm zeta_tm rho_tm Eq_tm s0)
+          (compRenRen_tm xi_tm zeta_tm rho_tm Eq_tm s1)
+          (compRenRen_tm xi_tm zeta_tm rho_tm Eq_tm s2)
+    | pair_tm _ s0 s1 =>
+        congr_pair_tm (compRenRen_tm xi_tm zeta_tm rho_tm Eq_tm s0)
+          (compRenRen_tm xi_tm zeta_tm rho_tm Eq_tm s1)
+    | pi1_tm _ s0 => congr_pi1_tm (compRenRen_tm xi_tm zeta_tm rho_tm Eq_tm s0)
+    | pi2_tm _ s0 => congr_pi2_tm (compRenRen_tm xi_tm zeta_tm rho_tm Eq_tm s0)
+    | imp_tm _ s0 s1 =>
+        congr_imp_tm (compRenRen_tm xi_tm zeta_tm rho_tm Eq_tm s0)
+          (compRenRen_tm xi_tm zeta_tm rho_tm Eq_tm s1)
+    | forall_tm _ s0 =>
+        congr_forall_tm
+          (compRenRen_tm (upRen_tm_tm xi_tm) (upRen_tm_tm zeta_tm)
+             (upRen_tm_tm rho_tm) (up_ren_ren _ _ _ Eq_tm) s0)
+    | sort_tm _ s0 s1 =>
+        congr_sort_tm (eq_refl s0)
+          (compRenRen_tm xi_tm zeta_tm rho_tm Eq_tm s1)
+    end.
+
+  Lemma up_ren_subst_tm_tm {k : nat} {l : nat} {m_tm : nat}
+    (xi : fin k -> fin l) (tau : fin l -> tm m_tm) (theta : fin k -> tm m_tm)
+    (Eq : forall x, funcomp tau xi x = theta x) :
+    forall x, funcomp (up_tm_tm tau) (upRen_tm_tm xi) x = up_tm_tm theta x.
+  Proof.
+    exact (fun n =>
+             match n with
+             | Some fin_n => ap (ren_tm shift) (Eq fin_n)
+             | None => eq_refl
+             end).
+  Qed.
+
+  Lemma up_ren_subst_list_tm_tm {p : nat} {k : nat} {l : nat} {m_tm : nat}
+    (xi : fin k -> fin l) (tau : fin l -> tm m_tm) (theta : fin k -> tm m_tm)
+    (Eq : forall x, funcomp tau xi x = theta x) :
+    forall x,
+      funcomp (up_list_tm_tm p tau) (upRen_list_tm_tm p xi) x =
+        up_list_tm_tm p theta x.
+  Proof.
+    exact (fun n =>
+             eq_trans (scons_p_comp' _ _ _ n)
+               (scons_p_congr (fun z => scons_p_head' _ _ z)
+                  (fun z =>
+                     eq_trans (scons_p_tail' _ _ (xi z))
+                       (ap (ren_tm (shift_p p)) (Eq z))))).
+  Qed.
+
+  Fixpoint compRenSubst_tm {k_tm : nat} {l_tm : nat} {m_tm : nat}
+    (xi_tm : fin m_tm -> fin k_tm) (tau_tm : fin k_tm -> tm l_tm)
+    (theta_tm : fin m_tm -> tm l_tm)
+    (Eq_tm : forall x, funcomp tau_tm xi_tm x = theta_tm x) (s : tm m_tm) {struct
+                                                                             s} : subst_tm tau_tm (ren_tm xi_tm s) = subst_tm theta_tm s :=
+    match s with
+    | var_tm _ s0 => Eq_tm s0
+    | lam_tm _ s0 =>
+        congr_lam_tm
+          (compRenSubst_tm (upRen_tm_tm xi_tm) (up_tm_tm tau_tm)
+             (up_tm_tm theta_tm) (up_ren_subst_tm_tm _ _ _ Eq_tm) s0)
+    | app_tm _ s0 s1 =>
+        congr_app_tm (compRenSubst_tm xi_tm tau_tm theta_tm Eq_tm s0)
+          (compRenSubst_tm xi_tm tau_tm theta_tm Eq_tm s1)
+    | z_tm _ => congr_z_tm
+    | s_tm _ s0 => congr_s_tm (compRenSubst_tm xi_tm tau_tm theta_tm Eq_tm s0)
+    | recN_tm _ s0 s1 s2 =>
+        congr_recN_tm (compRenSubst_tm xi_tm tau_tm theta_tm Eq_tm s0)
+          (compRenSubst_tm xi_tm tau_tm theta_tm Eq_tm s1)
+          (compRenSubst_tm xi_tm tau_tm theta_tm Eq_tm s2)
+    | tt_tm _ => congr_tt_tm
+    | ff_tm _ => congr_ff_tm
+    | recB_tm _ s0 s1 s2 =>
+        congr_recB_tm (compRenSubst_tm xi_tm tau_tm theta_tm Eq_tm s0)
+          (compRenSubst_tm xi_tm tau_tm theta_tm Eq_tm s1)
+          (compRenSubst_tm xi_tm tau_tm theta_tm Eq_tm s2)
+    | nil_tm _ => congr_nil_tm
+    | cons_tm _ s0 s1 =>
+        congr_cons_tm (compRenSubst_tm xi_tm tau_tm theta_tm Eq_tm s0)
+          (compRenSubst_tm xi_tm tau_tm theta_tm Eq_tm s1)
+    | recL_tm _ s0 s1 s2 =>
+        congr_recL_tm (compRenSubst_tm xi_tm tau_tm theta_tm Eq_tm s0)
+          (compRenSubst_tm xi_tm tau_tm theta_tm Eq_tm s1)
+          (compRenSubst_tm xi_tm tau_tm theta_tm Eq_tm s2)
+    | pair_tm _ s0 s1 =>
+        congr_pair_tm (compRenSubst_tm xi_tm tau_tm theta_tm Eq_tm s0)
+          (compRenSubst_tm xi_tm tau_tm theta_tm Eq_tm s1)
+    | pi1_tm _ s0 =>
+        congr_pi1_tm (compRenSubst_tm xi_tm tau_tm theta_tm Eq_tm s0)
+    | pi2_tm _ s0 =>
+        congr_pi2_tm (compRenSubst_tm xi_tm tau_tm theta_tm Eq_tm s0)
+    | imp_tm _ s0 s1 =>
+        congr_imp_tm (compRenSubst_tm xi_tm tau_tm theta_tm Eq_tm s0)
+          (compRenSubst_tm xi_tm tau_tm theta_tm Eq_tm s1)
+    | forall_tm _ s0 =>
+        congr_forall_tm
+          (compRenSubst_tm (upRen_tm_tm xi_tm) (up_tm_tm tau_tm)
+             (up_tm_tm theta_tm) (up_ren_subst_tm_tm _ _ _ Eq_tm) s0)
+    | sort_tm _ s0 s1 =>
+        congr_sort_tm (eq_refl s0)
+          (compRenSubst_tm xi_tm tau_tm theta_tm Eq_tm s1)
+    end.
+
+  Lemma up_subst_ren_tm_tm {k : nat} {l_tm : nat} {m_tm : nat}
+    (sigma : fin k -> tm l_tm) (zeta_tm : fin l_tm -> fin m_tm)
+    (theta : fin k -> tm m_tm)
+    (Eq : forall x, funcomp (ren_tm zeta_tm) sigma x = theta x) :
+    forall x,
+      funcomp (ren_tm (upRen_tm_tm zeta_tm)) (up_tm_tm sigma) x =
+        up_tm_tm theta x.
+  Proof.
+    exact (fun n =>
+             match n with
+             | Some fin_n =>
+                 eq_trans
+                   (compRenRen_tm shift (upRen_tm_tm zeta_tm)
+                      (funcomp shift zeta_tm) (fun x => eq_refl) (sigma fin_n))
+                   (eq_trans
+                      (eq_sym
+                         (compRenRen_tm zeta_tm shift (funcomp shift zeta_tm)
+                            (fun x => eq_refl) (sigma fin_n)))
+                      (ap (ren_tm shift) (Eq fin_n)))
+             | None => eq_refl
+             end).
+  Qed.
+
+  Lemma up_subst_ren_list_tm_tm {p : nat} {k : nat} {l_tm : nat} {m_tm : nat}
+    (sigma : fin k -> tm l_tm) (zeta_tm : fin l_tm -> fin m_tm)
+    (theta : fin k -> tm m_tm)
+    (Eq : forall x, funcomp (ren_tm zeta_tm) sigma x = theta x) :
+    forall x,
+      funcomp (ren_tm (upRen_list_tm_tm p zeta_tm)) (up_list_tm_tm p sigma) x =
+        up_list_tm_tm p theta x.
+  Proof.
+    exact (fun n =>
+             eq_trans (scons_p_comp' _ _ _ n)
+               (scons_p_congr
+                  (fun x => ap (var_tm (plus p m_tm)) (scons_p_head' _ _ x))
+                  (fun n =>
+                     eq_trans
+                       (compRenRen_tm (shift_p p) (upRen_list_tm_tm p zeta_tm)
+                          (funcomp (shift_p p) zeta_tm)
+                          (fun x => scons_p_tail' _ _ x) (sigma n))
+                       (eq_trans
+                          (eq_sym
+                             (compRenRen_tm zeta_tm (shift_p p)
+                                (funcomp (shift_p p) zeta_tm) (fun x => eq_refl)
+                                (sigma n))) (ap (ren_tm (shift_p p)) (Eq n)))))).
+  Qed.
+
+  Fixpoint compSubstRen_tm {k_tm : nat} {l_tm : nat} {m_tm : nat}
+    (sigma_tm : fin m_tm -> tm k_tm) (zeta_tm : fin k_tm -> fin l_tm)
+    (theta_tm : fin m_tm -> tm l_tm)
+    (Eq_tm : forall x, funcomp (ren_tm zeta_tm) sigma_tm x = theta_tm x)
+    (s : tm m_tm) {struct s} :
+    ren_tm zeta_tm (subst_tm sigma_tm s) = subst_tm theta_tm s :=
+    match s with
+    | var_tm _ s0 => Eq_tm s0
+    | lam_tm _ s0 =>
+        congr_lam_tm
+          (compSubstRen_tm (up_tm_tm sigma_tm) (upRen_tm_tm zeta_tm)
+             (up_tm_tm theta_tm) (up_subst_ren_tm_tm _ _ _ Eq_tm) s0)
+    | app_tm _ s0 s1 =>
+        congr_app_tm (compSubstRen_tm sigma_tm zeta_tm theta_tm Eq_tm s0)
+          (compSubstRen_tm sigma_tm zeta_tm theta_tm Eq_tm s1)
+    | z_tm _ => congr_z_tm
+    | s_tm _ s0 =>
+        congr_s_tm (compSubstRen_tm sigma_tm zeta_tm theta_tm Eq_tm s0)
+    | recN_tm _ s0 s1 s2 =>
+        congr_recN_tm (compSubstRen_tm sigma_tm zeta_tm theta_tm Eq_tm s0)
+          (compSubstRen_tm sigma_tm zeta_tm theta_tm Eq_tm s1)
+          (compSubstRen_tm sigma_tm zeta_tm theta_tm Eq_tm s2)
+    | tt_tm _ => congr_tt_tm
+    | ff_tm _ => congr_ff_tm
+    | recB_tm _ s0 s1 s2 =>
+        congr_recB_tm (compSubstRen_tm sigma_tm zeta_tm theta_tm Eq_tm s0)
+          (compSubstRen_tm sigma_tm zeta_tm theta_tm Eq_tm s1)
+          (compSubstRen_tm sigma_tm zeta_tm theta_tm Eq_tm s2)
+    | nil_tm _ => congr_nil_tm
+    | cons_tm _ s0 s1 =>
+        congr_cons_tm (compSubstRen_tm sigma_tm zeta_tm theta_tm Eq_tm s0)
+          (compSubstRen_tm sigma_tm zeta_tm theta_tm Eq_tm s1)
+    | recL_tm _ s0 s1 s2 =>
+        congr_recL_tm (compSubstRen_tm sigma_tm zeta_tm theta_tm Eq_tm s0)
+          (compSubstRen_tm sigma_tm zeta_tm theta_tm Eq_tm s1)
+          (compSubstRen_tm sigma_tm zeta_tm theta_tm Eq_tm s2)
+    | pair_tm _ s0 s1 =>
+        congr_pair_tm (compSubstRen_tm sigma_tm zeta_tm theta_tm Eq_tm s0)
+          (compSubstRen_tm sigma_tm zeta_tm theta_tm Eq_tm s1)
+    | pi1_tm _ s0 =>
+        congr_pi1_tm (compSubstRen_tm sigma_tm zeta_tm theta_tm Eq_tm s0)
+    | pi2_tm _ s0 =>
+        congr_pi2_tm (compSubstRen_tm sigma_tm zeta_tm theta_tm Eq_tm s0)
+    | imp_tm _ s0 s1 =>
+        congr_imp_tm (compSubstRen_tm sigma_tm zeta_tm theta_tm Eq_tm s0)
+          (compSubstRen_tm sigma_tm zeta_tm theta_tm Eq_tm s1)
+    | forall_tm _ s0 =>
+        congr_forall_tm
+          (compSubstRen_tm (up_tm_tm sigma_tm) (upRen_tm_tm zeta_tm)
+             (up_tm_tm theta_tm) (up_subst_ren_tm_tm _ _ _ Eq_tm) s0)
+    | sort_tm _ s0 s1 =>
+        congr_sort_tm (eq_refl s0)
+          (compSubstRen_tm sigma_tm zeta_tm theta_tm Eq_tm s1)
+    end.
+
+  Lemma up_subst_subst_tm_tm {k : nat} {l_tm : nat} {m_tm : nat}
+    (sigma : fin k -> tm l_tm) (tau_tm : fin l_tm -> tm m_tm)
+    (theta : fin k -> tm m_tm)
+    (Eq : forall x, funcomp (subst_tm tau_tm) sigma x = theta x) :
+    forall x,
+      funcomp (subst_tm (up_tm_tm tau_tm)) (up_tm_tm sigma) x = up_tm_tm theta x.
+  Proof.
+    exact (fun n =>
+             match n with
+             | Some fin_n =>
+                 eq_trans
+                   (compRenSubst_tm shift (up_tm_tm tau_tm)
+                      (funcomp (up_tm_tm tau_tm) shift) (fun x => eq_refl)
+                      (sigma fin_n))
+                   (eq_trans
+                      (eq_sym
+                         (compSubstRen_tm tau_tm shift
+                            (funcomp (ren_tm shift) tau_tm) (fun x => eq_refl)
+                            (sigma fin_n))) (ap (ren_tm shift) (Eq fin_n)))
+             | None => eq_refl
+             end).
+  Qed.
+
+  Lemma up_subst_subst_list_tm_tm {p : nat} {k : nat} {l_tm : nat} {m_tm : nat}
+    (sigma : fin k -> tm l_tm) (tau_tm : fin l_tm -> tm m_tm)
+    (theta : fin k -> tm m_tm)
+    (Eq : forall x, funcomp (subst_tm tau_tm) sigma x = theta x) :
+    forall x,
+      funcomp (subst_tm (up_list_tm_tm p tau_tm)) (up_list_tm_tm p sigma) x =
+        up_list_tm_tm p theta x.
+  Proof.
+    exact (fun n =>
+             eq_trans
+               (scons_p_comp' (funcomp (var_tm (plus p l_tm)) (zero_p p)) _ _ n)
+               (scons_p_congr
+                  (fun x => scons_p_head' _ (fun z => ren_tm (shift_p p) _) x)
+                  (fun n =>
+                     eq_trans
+                       (compRenSubst_tm (shift_p p) (up_list_tm_tm p tau_tm)
+                          (funcomp (up_list_tm_tm p tau_tm) (shift_p p))
+                          (fun x => eq_refl) (sigma n))
+                       (eq_trans
+                          (eq_sym
+                             (compSubstRen_tm tau_tm (shift_p p) _
+                                (fun x => eq_sym (scons_p_tail' _ _ x)) (sigma n)))
+                          (ap (ren_tm (shift_p p)) (Eq n)))))).
+  Qed.
+
+  Fixpoint compSubstSubst_tm {k_tm : nat} {l_tm : nat} {m_tm : nat}
+    (sigma_tm : fin m_tm -> tm k_tm) (tau_tm : fin k_tm -> tm l_tm)
+    (theta_tm : fin m_tm -> tm l_tm)
+    (Eq_tm : forall x, funcomp (subst_tm tau_tm) sigma_tm x = theta_tm x)
+    (s : tm m_tm) {struct s} :
+    subst_tm tau_tm (subst_tm sigma_tm s) = subst_tm theta_tm s :=
+    match s with
+    | var_tm _ s0 => Eq_tm s0
+    | lam_tm _ s0 =>
+        congr_lam_tm
+          (compSubstSubst_tm (up_tm_tm sigma_tm) (up_tm_tm tau_tm)
+             (up_tm_tm theta_tm) (up_subst_subst_tm_tm _ _ _ Eq_tm) s0)
+    | app_tm _ s0 s1 =>
+        congr_app_tm (compSubstSubst_tm sigma_tm tau_tm theta_tm Eq_tm s0)
+          (compSubstSubst_tm sigma_tm tau_tm theta_tm Eq_tm s1)
+    | z_tm _ => congr_z_tm
+    | s_tm _ s0 =>
+        congr_s_tm (compSubstSubst_tm sigma_tm tau_tm theta_tm Eq_tm s0)
+    | recN_tm _ s0 s1 s2 =>
+        congr_recN_tm (compSubstSubst_tm sigma_tm tau_tm theta_tm Eq_tm s0)
+          (compSubstSubst_tm sigma_tm tau_tm theta_tm Eq_tm s1)
+          (compSubstSubst_tm sigma_tm tau_tm theta_tm Eq_tm s2)
+    | tt_tm _ => congr_tt_tm
+    | ff_tm _ => congr_ff_tm
+    | recB_tm _ s0 s1 s2 =>
+        congr_recB_tm (compSubstSubst_tm sigma_tm tau_tm theta_tm Eq_tm s0)
+          (compSubstSubst_tm sigma_tm tau_tm theta_tm Eq_tm s1)
+          (compSubstSubst_tm sigma_tm tau_tm theta_tm Eq_tm s2)
+    | nil_tm _ => congr_nil_tm
+    | cons_tm _ s0 s1 =>
+        congr_cons_tm (compSubstSubst_tm sigma_tm tau_tm theta_tm Eq_tm s0)
+          (compSubstSubst_tm sigma_tm tau_tm theta_tm Eq_tm s1)
+    | recL_tm _ s0 s1 s2 =>
+        congr_recL_tm (compSubstSubst_tm sigma_tm tau_tm theta_tm Eq_tm s0)
+          (compSubstSubst_tm sigma_tm tau_tm theta_tm Eq_tm s1)
+          (compSubstSubst_tm sigma_tm tau_tm theta_tm Eq_tm s2)
+    | pair_tm _ s0 s1 =>
+        congr_pair_tm (compSubstSubst_tm sigma_tm tau_tm theta_tm Eq_tm s0)
+          (compSubstSubst_tm sigma_tm tau_tm theta_tm Eq_tm s1)
+    | pi1_tm _ s0 =>
+        congr_pi1_tm (compSubstSubst_tm sigma_tm tau_tm theta_tm Eq_tm s0)
+    | pi2_tm _ s0 =>
+        congr_pi2_tm (compSubstSubst_tm sigma_tm tau_tm theta_tm Eq_tm s0)
+    | imp_tm _ s0 s1 =>
+        congr_imp_tm (compSubstSubst_tm sigma_tm tau_tm theta_tm Eq_tm s0)
+          (compSubstSubst_tm sigma_tm tau_tm theta_tm Eq_tm s1)
+    | forall_tm _ s0 =>
+        congr_forall_tm
+          (compSubstSubst_tm (up_tm_tm sigma_tm) (up_tm_tm tau_tm)
+             (up_tm_tm theta_tm) (up_subst_subst_tm_tm _ _ _ Eq_tm) s0)
+    | sort_tm _ s0 s1 =>
+        congr_sort_tm (eq_refl s0)
+          (compSubstSubst_tm sigma_tm tau_tm theta_tm Eq_tm s1)
+    end.
+
+  Lemma renRen_tm {k_tm : nat} {l_tm : nat} {m_tm : nat}
+    (xi_tm : fin m_tm -> fin k_tm) (zeta_tm : fin k_tm -> fin l_tm)
+    (s : tm m_tm) :
+    ren_tm zeta_tm (ren_tm xi_tm s) = ren_tm (funcomp zeta_tm xi_tm) s.
+  Proof.
+    exact (compRenRen_tm xi_tm zeta_tm _ (fun n => eq_refl) s).
+  Qed.
+
+  Lemma renRen'_tm_pointwise {k_tm : nat} {l_tm : nat} {m_tm : nat}
+    (xi_tm : fin m_tm -> fin k_tm) (zeta_tm : fin k_tm -> fin l_tm) :
+    pointwise_relation _ eq (funcomp (ren_tm zeta_tm) (ren_tm xi_tm))
+      (ren_tm (funcomp zeta_tm xi_tm)).
+  Proof.
+    exact (fun s => compRenRen_tm xi_tm zeta_tm _ (fun n => eq_refl) s).
+  Qed.
+
+  Lemma renSubst_tm {k_tm : nat} {l_tm : nat} {m_tm : nat}
+    (xi_tm : fin m_tm -> fin k_tm) (tau_tm : fin k_tm -> tm l_tm) (s : tm m_tm)
+    : subst_tm tau_tm (ren_tm xi_tm s) = subst_tm (funcomp tau_tm xi_tm) s.
+  Proof.
+    exact (compRenSubst_tm xi_tm tau_tm _ (fun n => eq_refl) s).
+  Qed.
+
+  Lemma renSubst_tm_pointwise {k_tm : nat} {l_tm : nat} {m_tm : nat}
+    (xi_tm : fin m_tm -> fin k_tm) (tau_tm : fin k_tm -> tm l_tm) :
+    pointwise_relation _ eq (funcomp (subst_tm tau_tm) (ren_tm xi_tm))
+      (subst_tm (funcomp tau_tm xi_tm)).
+  Proof.
+    exact (fun s => compRenSubst_tm xi_tm tau_tm _ (fun n => eq_refl) s).
+  Qed.
+
+  Lemma substRen_tm {k_tm : nat} {l_tm : nat} {m_tm : nat}
+    (sigma_tm : fin m_tm -> tm k_tm) (zeta_tm : fin k_tm -> fin l_tm)
+    (s : tm m_tm) :
+    ren_tm zeta_tm (subst_tm sigma_tm s) =
+      subst_tm (funcomp (ren_tm zeta_tm) sigma_tm) s.
+  Proof.
+    exact (compSubstRen_tm sigma_tm zeta_tm _ (fun n => eq_refl) s).
+  Qed.
+
+  Lemma substRen_tm_pointwise {k_tm : nat} {l_tm : nat} {m_tm : nat}
+    (sigma_tm : fin m_tm -> tm k_tm) (zeta_tm : fin k_tm -> fin l_tm) :
+    pointwise_relation _ eq (funcomp (ren_tm zeta_tm) (subst_tm sigma_tm))
+      (subst_tm (funcomp (ren_tm zeta_tm) sigma_tm)).
+  Proof.
+    exact (fun s => compSubstRen_tm sigma_tm zeta_tm _ (fun n => eq_refl) s).
+  Qed.
+
+  Lemma substSubst_tm {k_tm : nat} {l_tm : nat} {m_tm : nat}
+    (sigma_tm : fin m_tm -> tm k_tm) (tau_tm : fin k_tm -> tm l_tm)
+    (s : tm m_tm) :
+    subst_tm tau_tm (subst_tm sigma_tm s) =
+      subst_tm (funcomp (subst_tm tau_tm) sigma_tm) s.
+  Proof.
+    exact (compSubstSubst_tm sigma_tm tau_tm _ (fun n => eq_refl) s).
+  Qed.
+
+  Lemma substSubst_tm_pointwise {k_tm : nat} {l_tm : nat} {m_tm : nat}
+    (sigma_tm : fin m_tm -> tm k_tm) (tau_tm : fin k_tm -> tm l_tm) :
+    pointwise_relation _ eq (funcomp (subst_tm tau_tm) (subst_tm sigma_tm))
+      (subst_tm (funcomp (subst_tm tau_tm) sigma_tm)).
+  Proof.
+    exact (fun s => compSubstSubst_tm sigma_tm tau_tm _ (fun n => eq_refl) s).
+  Qed.
+
+  Lemma rinstInst_up_tm_tm {m : nat} {n_tm : nat} (xi : fin m -> fin n_tm)
+    (sigma : fin m -> tm n_tm)
+    (Eq : forall x, funcomp (var_tm n_tm) xi x = sigma x) :
+    forall x, funcomp (var_tm (S n_tm)) (upRen_tm_tm xi) x = up_tm_tm sigma x.
+  Proof.
+    exact (fun n =>
+             match n with
+             | Some fin_n => ap (ren_tm shift) (Eq fin_n)
+             | None => eq_refl
+             end).
+  Qed.
+
+  Lemma rinstInst_up_list_tm_tm {p : nat} {m : nat} {n_tm : nat}
+    (xi : fin m -> fin n_tm) (sigma : fin m -> tm n_tm)
+    (Eq : forall x, funcomp (var_tm n_tm) xi x = sigma x) :
+    forall x,
+      funcomp (var_tm (plus p n_tm)) (upRen_list_tm_tm p xi) x =
+        up_list_tm_tm p sigma x.
+  Proof.
+    exact (fun n =>
+             eq_trans (scons_p_comp' _ _ (var_tm (plus p n_tm)) n)
+               (scons_p_congr (fun z => eq_refl)
+                  (fun n => ap (ren_tm (shift_p p)) (Eq n)))).
+  Qed.
+
+  Fixpoint rinst_inst_tm {m_tm : nat} {n_tm : nat}
+    (xi_tm : fin m_tm -> fin n_tm) (sigma_tm : fin m_tm -> tm n_tm)
+    (Eq_tm : forall x, funcomp (var_tm n_tm) xi_tm x = sigma_tm x) (s : tm m_tm)
+    {struct s} : ren_tm xi_tm s = subst_tm sigma_tm s :=
+    match s with
+    | var_tm _ s0 => Eq_tm s0
+    | lam_tm _ s0 =>
+        congr_lam_tm
+          (rinst_inst_tm (upRen_tm_tm xi_tm) (up_tm_tm sigma_tm)
+             (rinstInst_up_tm_tm _ _ Eq_tm) s0)
+    | app_tm _ s0 s1 =>
+        congr_app_tm (rinst_inst_tm xi_tm sigma_tm Eq_tm s0)
+          (rinst_inst_tm xi_tm sigma_tm Eq_tm s1)
+    | z_tm _ => congr_z_tm
+    | s_tm _ s0 => congr_s_tm (rinst_inst_tm xi_tm sigma_tm Eq_tm s0)
+    | recN_tm _ s0 s1 s2 =>
+        congr_recN_tm (rinst_inst_tm xi_tm sigma_tm Eq_tm s0)
+          (rinst_inst_tm xi_tm sigma_tm Eq_tm s1)
+          (rinst_inst_tm xi_tm sigma_tm Eq_tm s2)
+    | tt_tm _ => congr_tt_tm
+    | ff_tm _ => congr_ff_tm
+    | recB_tm _ s0 s1 s2 =>
+        congr_recB_tm (rinst_inst_tm xi_tm sigma_tm Eq_tm s0)
+          (rinst_inst_tm xi_tm sigma_tm Eq_tm s1)
+          (rinst_inst_tm xi_tm sigma_tm Eq_tm s2)
+    | nil_tm _ => congr_nil_tm
+    | cons_tm _ s0 s1 =>
+        congr_cons_tm (rinst_inst_tm xi_tm sigma_tm Eq_tm s0)
+          (rinst_inst_tm xi_tm sigma_tm Eq_tm s1)
+    | recL_tm _ s0 s1 s2 =>
+        congr_recL_tm (rinst_inst_tm xi_tm sigma_tm Eq_tm s0)
+          (rinst_inst_tm xi_tm sigma_tm Eq_tm s1)
+          (rinst_inst_tm xi_tm sigma_tm Eq_tm s2)
+    | pair_tm _ s0 s1 =>
+        congr_pair_tm (rinst_inst_tm xi_tm sigma_tm Eq_tm s0)
+          (rinst_inst_tm xi_tm sigma_tm Eq_tm s1)
+    | pi1_tm _ s0 => congr_pi1_tm (rinst_inst_tm xi_tm sigma_tm Eq_tm s0)
+    | pi2_tm _ s0 => congr_pi2_tm (rinst_inst_tm xi_tm sigma_tm Eq_tm s0)
+    | imp_tm _ s0 s1 =>
+        congr_imp_tm (rinst_inst_tm xi_tm sigma_tm Eq_tm s0)
+          (rinst_inst_tm xi_tm sigma_tm Eq_tm s1)
+    | forall_tm _ s0 =>
+        congr_forall_tm
+          (rinst_inst_tm (upRen_tm_tm xi_tm) (up_tm_tm sigma_tm)
+             (rinstInst_up_tm_tm _ _ Eq_tm) s0)
+    | sort_tm _ s0 s1 =>
+        congr_sort_tm (eq_refl s0) (rinst_inst_tm xi_tm sigma_tm Eq_tm s1)
+    end.
+
+  Lemma rinstInst'_tm {m_tm : nat} {n_tm : nat} (xi_tm : fin m_tm -> fin n_tm)
+    (s : tm m_tm) : ren_tm xi_tm s = subst_tm (funcomp (var_tm n_tm) xi_tm) s.
+  Proof.
+    exact (rinst_inst_tm xi_tm _ (fun n => eq_refl) s).
+  Qed.
+
+  Lemma rinstInst'_tm_pointwise {m_tm : nat} {n_tm : nat}
+    (xi_tm : fin m_tm -> fin n_tm) :
+    pointwise_relation _ eq (ren_tm xi_tm)
+      (subst_tm (funcomp (var_tm n_tm) xi_tm)).
+  Proof.
+    exact (fun s => rinst_inst_tm xi_tm _ (fun n => eq_refl) s).
+  Qed.
+
+  Lemma instId'_tm {m_tm : nat} (s : tm m_tm) : subst_tm (var_tm m_tm) s = s.
+  Proof.
+    exact (idSubst_tm (var_tm m_tm) (fun n => eq_refl) s).
+  Qed.
+
+  Lemma instId'_tm_pointwise {m_tm : nat} :
+    pointwise_relation _ eq (subst_tm (var_tm m_tm)) id.
+  Proof.
+    exact (fun s => idSubst_tm (var_tm m_tm) (fun n => eq_refl) s).
+  Qed.
+
+  Lemma rinstId'_tm {m_tm : nat} (s : tm m_tm) : ren_tm id s = s.
+  Proof.
+    exact (eq_ind_r (fun t => t = s) (instId'_tm s) (rinstInst'_tm id s)).
+  Qed.
+
+  Lemma rinstId'_tm_pointwise {m_tm : nat} :
+    pointwise_relation _ eq (@ren_tm m_tm m_tm id) id.
+  Proof.
+    exact (fun s => eq_ind_r (fun t => t = s) (instId'_tm s) (rinstInst'_tm id s)).
+  Qed.
+
+  Lemma varL'_tm {m_tm : nat} {n_tm : nat} (sigma_tm : fin m_tm -> tm n_tm)
+    (x : fin m_tm) : subst_tm sigma_tm (var_tm m_tm x) = sigma_tm x.
+  Proof.
+    exact (eq_refl).
+  Qed.
+
+  Lemma varL'_tm_pointwise {m_tm : nat} {n_tm : nat}
+    (sigma_tm : fin m_tm -> tm n_tm) :
+    pointwise_relation _ eq (funcomp (subst_tm sigma_tm) (var_tm m_tm))
+      sigma_tm.
+  Proof.
+    exact (fun x => eq_refl).
+  Qed.
+
+  Lemma varLRen'_tm {m_tm : nat} {n_tm : nat} (xi_tm : fin m_tm -> fin n_tm)
+    (x : fin m_tm) : ren_tm xi_tm (var_tm m_tm x) = var_tm n_tm (xi_tm x).
+  Proof.
+    exact (eq_refl).
+  Qed.
+
+  Lemma varLRen'_tm_pointwise {m_tm : nat} {n_tm : nat}
+    (xi_tm : fin m_tm -> fin n_tm) :
+    pointwise_relation _ eq (funcomp (ren_tm xi_tm) (var_tm m_tm))
+      (funcomp (var_tm n_tm) xi_tm).
+  Proof.
+    exact (fun x => eq_refl).
+  Qed.
+
+  Class Up_tm X Y :=
     up_tm : X -> Y.
 
-#[global] Instance Subst_tm : (Subst1 _ _ _) := @subst_tm.
+  #[global]
+    Instance Subst_tm  {m_tm n_tm : nat}: (Subst1 _ _ _) := (@subst_tm m_tm n_tm).
 
-#[global] Instance Up_tm_tm : (Up_tm _ _) := @up_tm_tm.
+  #[global]
+    Instance Up_tm_tm  {m n_tm : nat}: (Up_tm _ _) := (@up_tm_tm m n_tm).
 
-#[global] Instance Ren_tm : (Ren1 _ _ _) := @ren_tm.
+  #[global]
+    Instance Ren_tm  {m_tm n_tm : nat}: (Ren1 _ _ _) := (@ren_tm m_tm n_tm).
 
-#[global]
-Instance VarInstance_tm : (Var _ _) := @var_tm.
+  #[global]
+    Instance VarInstance_tm  {n_tm : nat}: (Var _ _) := (@var_tm n_tm).
 
-Notation "s [ sigma_tm ]" := (subst_tm sigma_tm s)
-( at level 7, left associativity, only printing)  : subst_scope.
+  Notation "s [ sigma_tm ]" := (subst_tm sigma_tm s)
+                                 ( at level 7, left associativity, only printing)  : subst_scope.
 
-Notation "↑__tm" := up_tm (only printing)  : subst_scope.
+  Notation "↑__tm" := up_tm (only printing)  : subst_scope.
 
-Notation "↑__tm" := up_tm_tm (only printing)  : subst_scope.
+  Notation "↑__tm" := up_tm_tm (only printing)  : subst_scope.
 
-Notation "s ⟨ xi_tm ⟩" := (ren_tm xi_tm s)
-( at level 7, left associativity, only printing)  : subst_scope.
+  Notation "s ⟨ xi_tm ⟩" := (ren_tm xi_tm s)
+                              ( at level 7, left associativity, only printing)  : subst_scope.
 
-Notation "'var'" := var_tm ( at level 1, only printing)  : subst_scope.
+  Notation "'var'" := var_tm ( at level 1, only printing)  : subst_scope.
 
-Notation "x '__tm'" := (@ids _ _ VarInstance_tm x)
-( at level 5, format "x __tm", only printing)  : subst_scope.
+  Notation "x '__tm'" := (@ids _ _ VarInstance_tm x)
+                           ( at level 5, format "x __tm", only printing)  : subst_scope.
 
-Notation "x '__tm'" := (var_tm x) ( at level 5, format "x __tm")  :
-subst_scope.
+  Notation "x '__tm'" := (var_tm x) ( at level 5, format "x __tm")  :
+      subst_scope.
 
-#[global]
-Instance subst_tm_morphism :
- (Proper (respectful (pointwise_relation _ eq) (respectful eq eq))
-    (@subst_tm)).
-Proof.
-exact (fun f_tm g_tm Eq_tm s t Eq_st =>
-       eq_ind s (fun t' => subst_tm f_tm s = subst_tm g_tm t')
-         (ext_tm f_tm g_tm Eq_tm s) t Eq_st).
-Qed.
+  #[global]
+    Instance subst_tm_morphism  {m_tm : nat} {n_tm : nat}:
+    (Proper (respectful (pointwise_relation _ eq) (respectful eq eq))
+       (@subst_tm m_tm n_tm)).
+  Proof.
+    exact (fun f_tm g_tm Eq_tm s t Eq_st =>
+             eq_ind s (fun t' => subst_tm f_tm s = subst_tm g_tm t')
+               (ext_tm f_tm g_tm Eq_tm s) t Eq_st).
+  Qed.
 
-#[global]
-Instance subst_tm_morphism2 :
- (Proper (respectful (pointwise_relation _ eq) (pointwise_relation _ eq))
-    (@subst_tm)).
-Proof.
-exact (fun f_tm g_tm Eq_tm s => ext_tm f_tm g_tm Eq_tm s).
-Qed.
+  #[global]
+    Instance subst_tm_morphism2  {m_tm : nat} {n_tm : nat}:
+    (Proper (respectful (pointwise_relation _ eq) (pointwise_relation _ eq))
+       (@subst_tm m_tm n_tm)).
+  Proof.
+    exact (fun f_tm g_tm Eq_tm s => ext_tm f_tm g_tm Eq_tm s).
+  Qed.
 
-#[global]
-Instance ren_tm_morphism :
- (Proper (respectful (pointwise_relation _ eq) (respectful eq eq)) (@ren_tm)).
-Proof.
-exact (fun f_tm g_tm Eq_tm s t Eq_st =>
-       eq_ind s (fun t' => ren_tm f_tm s = ren_tm g_tm t')
-         (extRen_tm f_tm g_tm Eq_tm s) t Eq_st).
-Qed.
+  #[global]
+    Instance ren_tm_morphism  {m_tm : nat} {n_tm : nat}:
+    (Proper (respectful (pointwise_relation _ eq) (respectful eq eq))
+       (@ren_tm m_tm n_tm)).
+  Proof.
+    exact (fun f_tm g_tm Eq_tm s t Eq_st =>
+             eq_ind s (fun t' => ren_tm f_tm s = ren_tm g_tm t')
+               (extRen_tm f_tm g_tm Eq_tm s) t Eq_st).
+  Qed.
 
-#[global]
-Instance ren_tm_morphism2 :
- (Proper (respectful (pointwise_relation _ eq) (pointwise_relation _ eq))
-    (@ren_tm)).
-Proof.
-exact (fun f_tm g_tm Eq_tm s => extRen_tm f_tm g_tm Eq_tm s).
-Qed.
+  #[global]
+    Instance ren_tm_morphism2  {m_tm : nat} {n_tm : nat}:
+    (Proper (respectful (pointwise_relation _ eq) (pointwise_relation _ eq))
+       (@ren_tm m_tm n_tm)).
+  Proof.
+    exact (fun f_tm g_tm Eq_tm s => extRen_tm f_tm g_tm Eq_tm s).
+  Qed.
 
-Ltac auto_unfold := repeat
-                     unfold VarInstance_tm, Var, ids, Ren_tm, Ren1, ren1,
-                      Up_tm_tm, Up_tm, up_tm, Subst_tm, Subst1, subst1.
+  Ltac auto_unfold := repeat
+                        unfold VarInstance_tm, Var, ids, Ren_tm, Ren1, ren1,
+      Up_tm_tm, Up_tm, up_tm, Subst_tm, Subst1, subst1.
 
-Tactic Notation "auto_unfold" "in" "*" := repeat
-                                           unfold VarInstance_tm, Var, ids,
-                                            Ren_tm, Ren1, ren1, Up_tm_tm,
-                                            Up_tm, up_tm, Subst_tm, Subst1,
-                                            subst1 in *.
+  Tactic Notation "auto_unfold" "in" "*" := repeat
+                                              unfold VarInstance_tm, Var, ids,
+      Ren_tm, Ren1, ren1, Up_tm_tm,
+      Up_tm, up_tm, Subst_tm, Subst1,
+      subst1 in *.
 
-Ltac asimpl' := repeat (first
-                 [ progress setoid_rewrite substSubst_tm_pointwise
-                 | progress setoid_rewrite substSubst_tm
-                 | progress setoid_rewrite substRen_tm_pointwise
-                 | progress setoid_rewrite substRen_tm
-                 | progress setoid_rewrite renSubst_tm_pointwise
-                 | progress setoid_rewrite renSubst_tm
-                 | progress setoid_rewrite renRen'_tm_pointwise
-                 | progress setoid_rewrite renRen_tm
-                 | progress setoid_rewrite varLRen'_tm_pointwise
-                 | progress setoid_rewrite varLRen'_tm
-                 | progress setoid_rewrite varL'_tm_pointwise
-                 | progress setoid_rewrite varL'_tm
-                 | progress setoid_rewrite rinstId'_tm_pointwise
-                 | progress setoid_rewrite rinstId'_tm
-                 | progress setoid_rewrite instId'_tm_pointwise
-                 | progress setoid_rewrite instId'_tm
-                 | progress unfold up_tm_tm, upRen_tm_tm, up_ren
-                 | progress cbn[subst_tm ren_tm]
-                 | progress fsimpl ]).
+  Ltac asimpl' := repeat (first
+                            [ progress setoid_rewrite substSubst_tm_pointwise
+                            | progress setoid_rewrite substSubst_tm
+                            | progress setoid_rewrite substRen_tm_pointwise
+                            | progress setoid_rewrite substRen_tm
+                            | progress setoid_rewrite renSubst_tm_pointwise
+                            | progress setoid_rewrite renSubst_tm
+                            | progress setoid_rewrite renRen'_tm_pointwise
+                            | progress setoid_rewrite renRen_tm
+                            | progress setoid_rewrite varLRen'_tm_pointwise
+                            | progress setoid_rewrite varLRen'_tm
+                            | progress setoid_rewrite varL'_tm_pointwise
+                            | progress setoid_rewrite varL'_tm
+                            | progress setoid_rewrite rinstId'_tm_pointwise
+                            | progress setoid_rewrite rinstId'_tm
+                            | progress setoid_rewrite instId'_tm_pointwise
+                            | progress setoid_rewrite instId'_tm
+                            | progress
+                                unfold up_list_tm_tm, up_tm_tm, upRen_list_tm_tm,
+                              upRen_tm_tm, up_ren
+                            | progress cbn[subst_tm ren_tm]
+                            | progress fsimpl ]).
 
-Ltac asimpl := check_no_evars;
-                repeat
-                 unfold VarInstance_tm, Var, ids, Ren_tm, Ren1, ren1,
-                  Up_tm_tm, Up_tm, up_tm, Subst_tm, Subst1, subst1 in *;
-                asimpl'; minimize.
+  Ltac asimpl := check_no_evars;
+                 repeat
+                   unfold VarInstance_tm, Var, ids, Ren_tm, Ren1, ren1,
+                   Up_tm_tm, Up_tm, up_tm, Subst_tm, Subst1, subst1 in *;
+                 asimpl'; minimize.
 
-Tactic Notation "asimpl" "in" hyp(J) := revert J; asimpl; intros J.
+  Tactic Notation "asimpl" "in" hyp(J) := revert J; asimpl; intros J.
 
-Tactic Notation "auto_case" := auto_case ltac:(asimpl; cbn; eauto).
+  Tactic Notation "auto_case" := auto_case ltac:(asimpl; cbn; eauto).
 
-Ltac substify := auto_unfold; try setoid_rewrite rinstInst'_tm_pointwise;
-                  try setoid_rewrite rinstInst'_tm.
+  Ltac substify := auto_unfold; try setoid_rewrite rinstInst'_tm_pointwise;
+                   try setoid_rewrite rinstInst'_tm.
 
-Ltac renamify := auto_unfold; try setoid_rewrite_left rinstInst'_tm_pointwise;
-                  try setoid_rewrite_left rinstInst'_tm.
+  Ltac renamify := auto_unfold; try setoid_rewrite_left rinstInst'_tm_pointwise;
+                   try setoid_rewrite_left rinstInst'_tm.
 
 End Core.
 
 Module Extra.
 
-Import Core.
+  Import
+    Core.
 
-#[global] Hint Opaque subst_tm: rewrite.
+  Arguments var_tm {n_tm}.
 
-#[global] Hint Opaque ren_tm: rewrite.
+  Arguments sort_tm {n_tm}.
+
+  Arguments forall_tm {n_tm}.
+
+  Arguments imp_tm {n_tm}.
+
+  Arguments pi2_tm {n_tm}.
+
+  Arguments pi1_tm {n_tm}.
+
+  Arguments pair_tm {n_tm}.
+
+  Arguments recL_tm {n_tm}.
+
+  Arguments cons_tm {n_tm}.
+
+  Arguments nil_tm {n_tm}.
+
+  Arguments recB_tm {n_tm}.
+
+  Arguments ff_tm {n_tm}.
+
+  Arguments tt_tm {n_tm}.
+
+  Arguments recN_tm {n_tm}.
+
+  Arguments s_tm {n_tm}.
+
+  Arguments z_tm {n_tm}.
+
+  Arguments app_tm {n_tm}.
+
+  Arguments lam_tm {n_tm}.
+
+  #[global] Hint Opaque subst_tm: rewrite.
+
+  #[global] Hint Opaque ren_tm: rewrite.
 
 End Extra.
 
 Module interface.
 
-Export Core.
+  Export Core.
 
-Export Extra.
+  Export Extra.
 
 End interface.
 
